QCP_examples/humaneval/spec_logic_rewrite_c_files/C_154_goal.v
@@ -1,0 +1,1255 @@
+Require Import Coq.ZArith.ZArith.
+Require Import Coq.Bool.Bool.
+Require Import Coq.Strings.String.
+Require Import Coq.Strings.Ascii.
+Require Import Coq.Lists.List.
+Require Import Coq.Classes.RelationClasses.
+Require Import Coq.Classes.Morphisms.
+Require Import Coq.micromega.Psatz.
+Require Import Coq.Sorting.Permutation.
+From AUXLib Require Import int_auto Axioms Feq Idents ListLib VMap.
+Require Import SetsClass.SetsClass. Import SetsNotation.
+From SimpleC.SL Require Import Mem SeparationLogic.
+Require Import Logic.LogicGenerator.demo932.Interface.
+Local Open Scope Z_scope.
+Local Open Scope sets.
+Local Open Scope string_scope.
+Local Open Scope list.
+Import naive_C_Rules.
+Require Import SimpleC.StdLib.string_lib.
+Require Import coins_154.
+Local Open Scope sac.
+From SimpleC.EE.QCP_demos_LLM Require Import char_array_strategy_goal.
+From SimpleC.EE.QCP_demos_LLM Require Import char_array_strategy_proof.
+From SimpleC.StdLib Require Import string_strategy_goal.
+From SimpleC.StdLib Require Import string_strategy_proof.
+
+(*----- Function cycpattern_check -----*)
+
+Definition cycpattern_check_safety_wit_1 := 
+forall (b_pre: Z) (a_pre: Z) (b0: Z) (a0: Z) (b_l: (@list Z)) (a_l: (@list Z)) (retval: Z) (PreH1 : (retval = (string_length (b_l)))) (PreH2 : (0 <= ((string_length (b_l)) + 1 ))) (PreH3 : (0 <= ((string_length (a_l)) + 1 ))) (PreH4 : (a_pre = a0)) (PreH5 : (b_pre = b0)) (PreH6 : (problem_154_pre_z a_l b_l )) (PreH7 : (valid_string a_l )) (PreH8 : (valid_string b_l )) (PreH9 : ((string_length (a_l)) < INT_MAX)) (PreH10 : (((string_length (b_l)) + 1 ) < INT_MAX)) ,
+  ((( &( "rotate" ) )) # Ptr  |->_)
+  **  (store_string b_pre b_l )
+  **  (CharArray.full a0 ((string_length (a_l)) + 1 ) (c_string (a_l)) )
+  **  ((( &( "n" ) )) # Int  |-> retval)
+  **  ((( &( "b" ) )) # Ptr  |-> b_pre)
+  **  ((( &( "a" ) )) # Ptr  |-> a_pre)
+|--
+  “ ((retval + 1 ) <= INT_MAX) ” 
+  &&  “ ((INT_MIN) <= (retval + 1 )) ”
+.
+
+Definition cycpattern_check_safety_wit_2 := 
+forall (b_pre: Z) (a_pre: Z) (b0: Z) (a0: Z) (b_l: (@list Z)) (a_l: (@list Z)) (retval: Z) (PreH1 : (retval = (string_length (b_l)))) (PreH2 : (0 <= ((string_length (b_l)) + 1 ))) (PreH3 : (0 <= ((string_length (a_l)) + 1 ))) (PreH4 : (a_pre = a0)) (PreH5 : (b_pre = b0)) (PreH6 : (problem_154_pre_z a_l b_l )) (PreH7 : (valid_string a_l )) (PreH8 : (valid_string b_l )) (PreH9 : ((string_length (a_l)) < INT_MAX)) (PreH10 : (((string_length (b_l)) + 1 ) < INT_MAX)) ,
+  ((( &( "rotate" ) )) # Ptr  |->_)
+  **  (store_string b_pre b_l )
+  **  (CharArray.full a0 ((string_length (a_l)) + 1 ) (c_string (a_l)) )
+  **  ((( &( "n" ) )) # Int  |-> retval)
+  **  ((( &( "b" ) )) # Ptr  |-> b_pre)
+  **  ((( &( "a" ) )) # Ptr  |-> a_pre)
+|--
+  “ (1 <= INT_MAX) ” 
+  &&  “ ((INT_MIN) <= 1) ”
+.
+
+Definition cycpattern_check_safety_wit_3 := 
+forall (b_pre: Z) (a_pre: Z) (b0: Z) (a0: Z) (b_l: (@list Z)) (a_l: (@list Z)) (retval: Z) (retval_2: Z) (PreH1 : (retval_2 <> 0)) (PreH2 : (retval = (string_length (b_l)))) (PreH3 : (0 <= ((string_length (b_l)) + 1 ))) (PreH4 : (0 <= ((string_length (a_l)) + 1 ))) (PreH5 : (a_pre = a0)) (PreH6 : (b_pre = b0)) (PreH7 : (problem_154_pre_z a_l b_l )) (PreH8 : (valid_string a_l )) (PreH9 : (valid_string b_l )) (PreH10 : ((string_length (a_l)) < INT_MAX)) (PreH11 : (((string_length (b_l)) + 1 ) < INT_MAX)) ,
+  (CharArray.undef_full retval_2 (retval + 1 ) )
+  **  (CharArray.full b_pre ((string_length (b_l)) + 1 ) (c_string (b_l)) )
+  **  ((( &( "rotate" ) )) # Ptr  |-> retval_2)
+  **  (CharArray.full a0 ((string_length (a_l)) + 1 ) (c_string (a_l)) )
+  **  ((( &( "n" ) )) # Int  |-> retval)
+  **  ((( &( "b" ) )) # Ptr  |-> b_pre)
+  **  ((( &( "a" ) )) # Ptr  |-> a_pre)
+|--
+  “ (0 <= INT_MAX) ” 
+  &&  “ ((INT_MIN) <= 0) ”
+.
+
+Definition cycpattern_check_safety_wit_4 := 
+forall (b_pre: Z) (a_pre: Z) (b0: Z) (a0: Z) (b_l: (@list Z)) (a_l: (@list Z)) (retval: Z) (retval_2: Z) (PreH1 : (retval_2 = 0)) (PreH2 : (retval_2 <> 0)) (PreH3 : (retval = (string_length (b_l)))) (PreH4 : (0 <= ((string_length (b_l)) + 1 ))) (PreH5 : (0 <= ((string_length (a_l)) + 1 ))) (PreH6 : (a_pre = a0)) (PreH7 : (b_pre = b0)) (PreH8 : (problem_154_pre_z a_l b_l )) (PreH9 : (valid_string a_l )) (PreH10 : (valid_string b_l )) (PreH11 : ((string_length (a_l)) < INT_MAX)) (PreH12 : (((string_length (b_l)) + 1 ) < INT_MAX)) ,
+  (CharArray.undef_full retval_2 (retval + 1 ) )
+  **  (CharArray.full b_pre ((string_length (b_l)) + 1 ) (c_string (b_l)) )
+  **  ((( &( "rotate" ) )) # Ptr  |-> retval_2)
+  **  (CharArray.full a0 ((string_length (a_l)) + 1 ) (c_string (a_l)) )
+  **  ((( &( "n" ) )) # Int  |-> retval)
+  **  ((( &( "b" ) )) # Ptr  |-> b_pre)
+  **  ((( &( "a" ) )) # Ptr  |-> a_pre)
+|--
+  “ False ”
+.
+
+Definition cycpattern_check_safety_wit_5 := 
+forall (b_pre: Z) (a_pre: Z) (b0: Z) (a0: Z) (b_l: (@list Z)) (a_l: (@list Z)) (retval: Z) (retval_2: Z) (PreH1 : (retval_2 <> 0)) (PreH2 : (retval_2 <> 0)) (PreH3 : (retval = (string_length (b_l)))) (PreH4 : (0 <= ((string_length (b_l)) + 1 ))) (PreH5 : (0 <= ((string_length (a_l)) + 1 ))) (PreH6 : (a_pre = a0)) (PreH7 : (b_pre = b0)) (PreH8 : (problem_154_pre_z a_l b_l )) (PreH9 : (valid_string a_l )) (PreH10 : (valid_string b_l )) (PreH11 : ((string_length (a_l)) < INT_MAX)) (PreH12 : (((string_length (b_l)) + 1 ) < INT_MAX)) ,
+  ((( &( "i" ) )) # Int  |->_)
+  **  (CharArray.undef_full retval_2 (retval + 1 ) )
+  **  (CharArray.full b_pre ((string_length (b_l)) + 1 ) (c_string (b_l)) )
+  **  ((( &( "rotate" ) )) # Ptr  |-> retval_2)
+  **  (CharArray.full a0 ((string_length (a_l)) + 1 ) (c_string (a_l)) )
+  **  ((( &( "n" ) )) # Int  |-> retval)
+  **  ((( &( "b" ) )) # Ptr  |-> b_pre)
+  **  ((( &( "a" ) )) # Ptr  |-> a_pre)
+|--
+  “ (0 <= INT_MAX) ” 
+  &&  “ ((INT_MIN) <= 0) ”
+.
+
+Definition cycpattern_check_safety_wit_6 := 
+forall (b0: Z) (a0: Z) (b_l: (@list Z)) (a_l: (@list Z)) (rotate: Z) (n: Z) (i: Z) (PreH1 : (i < n)) (PreH2 : (0 <= i)) (PreH3 : (i <= n)) (PreH4 : (rotate <> 0)) (PreH5 : ((n + 1 ) < INT_MAX)) (PreH6 : (valid_string a_l )) (PreH7 : (valid_string b_l )) (PreH8 : ((string_length (a_l)) < INT_MAX)) (PreH9 : (n = (string_length (b_l)))) (PreH10 : (rotation_scan_state_154 a_l b_l i )) ,
+  ((( &( "j" ) )) # Int  |->_)
+  **  ((( &( "i" ) )) # Int  |-> i)
+  **  ((( &( "n" ) )) # Int  |-> n)
+  **  ((( &( "rotate" ) )) # Ptr  |-> rotate)
+  **  ((( &( "a" ) )) # Ptr  |-> a0)
+  **  ((( &( "b" ) )) # Ptr  |-> b0)
+  **  (store_string a0 a_l )
+  **  (store_string b0 b_l )
+  **  (CharArray.undef_full rotate (n + 1 ) )
+|--
+  “ (0 <= INT_MAX) ” 
+  &&  “ ((INT_MIN) <= 0) ”
+.
+
+Definition cycpattern_check_safety_wit_7 := 
+forall (b0: Z) (a0: Z) (b_l: (@list Z)) (a_l: (@list Z)) (rotate_l: (@list Z)) (rotate: Z) (i: Z) (n: Z) (j: Z) (PreH1 : (j < n)) (PreH2 : (0 <= j)) (PreH3 : (j <= n)) (PreH4 : (0 < n)) (PreH5 : (0 <= i)) (PreH6 : (i < n)) (PreH7 : (rotate <> 0)) (PreH8 : ((n + 1 ) < INT_MAX)) (PreH9 : (valid_string a_l )) (PreH10 : (valid_string b_l )) (PreH11 : ((string_length (a_l)) < INT_MAX)) (PreH12 : (n = (string_length (b_l)))) (PreH13 : (rotation_scan_state_154 a_l b_l i )) (PreH14 : (rotation_prefix_154 b_l i j rotate_l )) ,
+  ((( &( "idx" ) )) # Int  |->_)
+  **  ((( &( "j" ) )) # Int  |-> j)
+  **  ((( &( "n" ) )) # Int  |-> n)
+  **  ((( &( "i" ) )) # Int  |-> i)
+  **  ((( &( "rotate" ) )) # Ptr  |-> rotate)
+  **  ((( &( "a" ) )) # Ptr  |-> a0)
+  **  ((( &( "b" ) )) # Ptr  |-> b0)
+  **  (store_string a0 a_l )
+  **  (store_string b0 b_l )
+  **  (CharArray.full rotate j rotate_l )
+  **  (CharArray.undef_seg rotate j (n + 1 ) )
+|--
+  “ ((n - i ) <= INT_MAX) ” 
+  &&  “ ((INT_MIN) <= (n - i )) ”
+.
+
+Definition cycpattern_check_safety_wit_8 := 
+forall (b0: Z) (a0: Z) (b_l: (@list Z)) (a_l: (@list Z)) (rotate_l: (@list Z)) (rotate: Z) (i: Z) (n: Z) (j: Z) (PreH1 : (j >= (n - i ))) (PreH2 : (j < n)) (PreH3 : (0 <= j)) (PreH4 : (j <= n)) (PreH5 : (0 < n)) (PreH6 : (0 <= i)) (PreH7 : (i < n)) (PreH8 : (rotate <> 0)) (PreH9 : ((n + 1 ) < INT_MAX)) (PreH10 : (valid_string a_l )) (PreH11 : (valid_string b_l )) (PreH12 : ((string_length (a_l)) < INT_MAX)) (PreH13 : (n = (string_length (b_l)))) (PreH14 : (rotation_scan_state_154 a_l b_l i )) (PreH15 : (rotation_prefix_154 b_l i j rotate_l )) ,
+  ((( &( "idx" ) )) # Int  |->_)
+  **  ((( &( "j" ) )) # Int  |-> j)
+  **  ((( &( "n" ) )) # Int  |-> n)
+  **  ((( &( "i" ) )) # Int  |-> i)
+  **  ((( &( "rotate" ) )) # Ptr  |-> rotate)
+  **  ((( &( "a" ) )) # Ptr  |-> a0)
+  **  ((( &( "b" ) )) # Ptr  |-> b0)
+  **  (store_string a0 a_l )
+  **  (store_string b0 b_l )
+  **  (CharArray.full rotate j rotate_l )
+  **  (CharArray.undef_seg rotate j (n + 1 ) )
+|--
+  “ ((j - (n - i ) ) <= INT_MAX) ” 
+  &&  “ ((INT_MIN) <= (j - (n - i ) )) ”
+.
+
+Definition cycpattern_check_safety_wit_9 := 
+forall (b0: Z) (a0: Z) (b_l: (@list Z)) (a_l: (@list Z)) (rotate_l: (@list Z)) (rotate: Z) (i: Z) (n: Z) (j: Z) (PreH1 : (j >= (n - i ))) (PreH2 : (j < n)) (PreH3 : (0 <= j)) (PreH4 : (j <= n)) (PreH5 : (0 < n)) (PreH6 : (0 <= i)) (PreH7 : (i < n)) (PreH8 : (rotate <> 0)) (PreH9 : ((n + 1 ) < INT_MAX)) (PreH10 : (valid_string a_l )) (PreH11 : (valid_string b_l )) (PreH12 : ((string_length (a_l)) < INT_MAX)) (PreH13 : (n = (string_length (b_l)))) (PreH14 : (rotation_scan_state_154 a_l b_l i )) (PreH15 : (rotation_prefix_154 b_l i j rotate_l )) ,
+  ((( &( "idx" ) )) # Int  |->_)
+  **  ((( &( "j" ) )) # Int  |-> j)
+  **  ((( &( "n" ) )) # Int  |-> n)
+  **  ((( &( "i" ) )) # Int  |-> i)
+  **  ((( &( "rotate" ) )) # Ptr  |-> rotate)
+  **  ((( &( "a" ) )) # Ptr  |-> a0)
+  **  ((( &( "b" ) )) # Ptr  |-> b0)
+  **  (store_string a0 a_l )
+  **  (store_string b0 b_l )
+  **  (CharArray.full rotate j rotate_l )
+  **  (CharArray.undef_seg rotate j (n + 1 ) )
+|--
+  “ ((n - i ) <= INT_MAX) ” 
+  &&  “ ((INT_MIN) <= (n - i )) ”
+.
+
+Definition cycpattern_check_safety_wit_10 := 
+forall (b0: Z) (a0: Z) (b_l: (@list Z)) (a_l: (@list Z)) (rotate_l: (@list Z)) (rotate: Z) (i: Z) (n: Z) (j: Z) (PreH1 : (j < (n - i ))) (PreH2 : (j < n)) (PreH3 : (0 <= j)) (PreH4 : (j <= n)) (PreH5 : (0 < n)) (PreH6 : (0 <= i)) (PreH7 : (i < n)) (PreH8 : (rotate <> 0)) (PreH9 : ((n + 1 ) < INT_MAX)) (PreH10 : (valid_string a_l )) (PreH11 : (valid_string b_l )) (PreH12 : ((string_length (a_l)) < INT_MAX)) (PreH13 : (n = (string_length (b_l)))) (PreH14 : (rotation_scan_state_154 a_l b_l i )) (PreH15 : (rotation_prefix_154 b_l i j rotate_l )) ,
+  ((( &( "idx" ) )) # Int  |->_)
+  **  ((( &( "j" ) )) # Int  |-> j)
+  **  ((( &( "n" ) )) # Int  |-> n)
+  **  ((( &( "i" ) )) # Int  |-> i)
+  **  ((( &( "rotate" ) )) # Ptr  |-> rotate)
+  **  ((( &( "a" ) )) # Ptr  |-> a0)
+  **  ((( &( "b" ) )) # Ptr  |-> b0)
+  **  (store_string a0 a_l )
+  **  (store_string b0 b_l )
+  **  (CharArray.full rotate j rotate_l )
+  **  (CharArray.undef_seg rotate j (n + 1 ) )
+|--
+  “ ((i + j ) <= INT_MAX) ” 
+  &&  “ ((INT_MIN) <= (i + j )) ”
+.
+
+Definition cycpattern_check_safety_wit_11 := 
+forall (b0: Z) (a0: Z) (b_l: (@list Z)) (a_l: (@list Z)) (rotate_l: (@list Z)) (ch: Z) (idx: Z) (i: Z) (j: Z) (n: Z) (rotate: Z) (PreH1 : (0 <= ((string_length (b_l)) + 1 ))) (PreH2 : (0 <= ((string_length (a_l)) + 1 ))) (PreH3 : (ch = (Znth (idx) (b_l) (0)))) (PreH4 : (idx = ((i + j ) % ( n ) ))) (PreH5 : (0 <= ch)) (PreH6 : (ch <= 127)) (PreH7 : (0 <= idx)) (PreH8 : (idx < n)) (PreH9 : (0 <= j)) (PreH10 : (j < n)) (PreH11 : (0 < n)) (PreH12 : (0 <= i)) (PreH13 : (i < n)) (PreH14 : (rotate <> 0)) (PreH15 : ((n + 1 ) < INT_MAX)) (PreH16 : (valid_string a_l )) (PreH17 : (valid_string b_l )) (PreH18 : ((string_length (a_l)) < INT_MAX)) (PreH19 : (n = (string_length (b_l)))) (PreH20 : (rotation_scan_state_154 a_l b_l i )) (PreH21 : (rotation_prefix_154 b_l i j rotate_l )) ,
+  (CharArray.full rotate (j + 1 ) (app (rotate_l) ((cons (ch) ((@nil Z))))) )
+  **  (CharArray.undef_seg rotate (j + 1 ) (n + 1 ) )
+  **  (CharArray.full b0 ((string_length (b_l)) + 1 ) (c_string (b_l)) )
+  **  (CharArray.full a0 ((string_length (a_l)) + 1 ) (c_string (a_l)) )
+  **  ((( &( "i" ) )) # Int  |-> i)
+  **  ((( &( "j" ) )) # Int  |-> j)
+  **  ((( &( "n" ) )) # Int  |-> n)
+  **  ((( &( "rotate" ) )) # Ptr  |-> rotate)
+  **  ((( &( "a" ) )) # Ptr  |-> a0)
+  **  ((( &( "b" ) )) # Ptr  |-> b0)
+|--
+  “ ((j + 1 ) <= INT_MAX) ” 
+  &&  “ ((INT_MIN) <= (j + 1 )) ”
+.
+
+Definition cycpattern_check_safety_wit_12 := 
+forall (b0: Z) (a0: Z) (b_l: (@list Z)) (a_l: (@list Z)) (rotate_l: (@list Z)) (rotate: Z) (i: Z) (n: Z) (j: Z) (PreH1 : (j >= n)) (PreH2 : (0 <= j)) (PreH3 : (j <= n)) (PreH4 : (0 < n)) (PreH5 : (0 <= i)) (PreH6 : (i < n)) (PreH7 : (rotate <> 0)) (PreH8 : ((n + 1 ) < INT_MAX)) (PreH9 : (valid_string a_l )) (PreH10 : (valid_string b_l )) (PreH11 : ((string_length (a_l)) < INT_MAX)) (PreH12 : (n = (string_length (b_l)))) (PreH13 : (rotation_scan_state_154 a_l b_l i )) (PreH14 : (rotation_prefix_154 b_l i j rotate_l )) ,
+  ((( &( "n" ) )) # Int  |-> n)
+  **  ((( &( "i" ) )) # Int  |-> i)
+  **  ((( &( "rotate" ) )) # Ptr  |-> rotate)
+  **  ((( &( "a" ) )) # Ptr  |-> a0)
+  **  ((( &( "b" ) )) # Ptr  |-> b0)
+  **  (store_string a0 a_l )
+  **  (store_string b0 b_l )
+  **  (CharArray.full rotate j rotate_l )
+  **  (CharArray.undef_seg rotate j (n + 1 ) )
+|--
+  “ (0 <= INT_MAX) ” 
+  &&  “ ((INT_MIN) <= 0) ”
+.
+
+Definition cycpattern_check_safety_wit_13 := 
+forall (b0: Z) (a0: Z) (b_l: (@list Z)) (a_l: (@list Z)) (rotate: Z) (n: Z) (i: Z) (retval: Z) (PreH1 : (strstr_result a_l (rotate_at_154 (b_l) (i)) retval a0 )) (PreH2 : (0 <= ((string_length ((rotate_at_154 (b_l) (i)))) + 1 ))) (PreH3 : (0 <= ((string_length (b_l)) + 1 ))) (PreH4 : (0 <= ((string_length (a_l)) + 1 ))) (PreH5 : (rotate <> 0)) (PreH6 : ((n + 1 ) < INT_MAX)) (PreH7 : (valid_string a_l )) (PreH8 : (valid_string b_l )) (PreH9 : ((string_length (a_l)) < INT_MAX)) (PreH10 : (n = (string_length (b_l)))) (PreH11 : (rotation_scan_state_154 a_l b_l i )) (PreH12 : (rotation_prefix_154 b_l i n (rotate_at_154 (b_l) (i)) )) (PreH13 : (valid_string (rotate_at_154 (b_l) (i)) )) ,
+  (store_string a0 a_l )
+  **  (store_string rotate (rotate_at_154 (b_l) (i)) )
+  **  (CharArray.full b0 ((string_length (b_l)) + 1 ) (c_string (b_l)) )
+  **  ((( &( "hit" ) )) # Ptr  |-> retval)
+  **  ((( &( "rotate" ) )) # Ptr  |-> rotate)
+  **  ((( &( "n" ) )) # Int  |-> n)
+  **  ((( &( "a" ) )) # Ptr  |-> a0)
+  **  ((( &( "b" ) )) # Ptr  |-> b0)
+  **  ((( &( "i" ) )) # Int  |-> i)
+|--
+  “ (0 <= INT_MAX) ” 
+  &&  “ ((INT_MIN) <= 0) ”
+.
+
+Definition cycpattern_check_safety_wit_14 := 
+forall (b0: Z) (a0: Z) (b_l: (@list Z)) (a_l: (@list Z)) (hit: Z) (rotate: Z) (n: Z) (i: Z) (PreH1 : (hit <> 0)) (PreH2 : (rotate <> 0)) (PreH3 : ((n + 1 ) < INT_MAX)) (PreH4 : (valid_string a_l )) (PreH5 : (valid_string b_l )) (PreH6 : ((string_length (a_l)) < INT_MAX)) (PreH7 : (n = (string_length (b_l)))) (PreH8 : (rotation_success_154 a_l b_l i (rotate_at_154 (b_l) (i)) )) ,
+  ((( &( "hit" ) )) # Ptr  |-> hit)
+  **  ((( &( "rotate" ) )) # Ptr  |-> rotate)
+  **  ((( &( "n" ) )) # Int  |-> n)
+  **  ((( &( "a" ) )) # Ptr  |-> a0)
+  **  ((( &( "b" ) )) # Ptr  |-> b0)
+  **  ((( &( "i" ) )) # Int  |-> i)
+  **  (store_string a0 a_l )
+  **  (store_string b0 b_l )
+  **  (CharArray.undef_full rotate (n + 1 ) )
+|--
+  “ ((n + 1 ) <= INT_MAX) ” 
+  &&  “ ((INT_MIN) <= (n + 1 )) ”
+.
+
+Definition cycpattern_check_safety_wit_15 := 
+forall (b0: Z) (a0: Z) (b_l: (@list Z)) (a_l: (@list Z)) (hit: Z) (rotate: Z) (n: Z) (i: Z) (PreH1 : (hit <> 0)) (PreH2 : (rotate <> 0)) (PreH3 : ((n + 1 ) < INT_MAX)) (PreH4 : (valid_string a_l )) (PreH5 : (valid_string b_l )) (PreH6 : ((string_length (a_l)) < INT_MAX)) (PreH7 : (n = (string_length (b_l)))) (PreH8 : (rotation_success_154 a_l b_l i (rotate_at_154 (b_l) (i)) )) ,
+  ((( &( "hit" ) )) # Ptr  |-> hit)
+  **  ((( &( "rotate" ) )) # Ptr  |-> rotate)
+  **  ((( &( "n" ) )) # Int  |-> n)
+  **  ((( &( "a" ) )) # Ptr  |-> a0)
+  **  ((( &( "b" ) )) # Ptr  |-> b0)
+  **  ((( &( "i" ) )) # Int  |-> i)
+  **  (store_string a0 a_l )
+  **  (store_string b0 b_l )
+  **  (CharArray.undef_full rotate (n + 1 ) )
+|--
+  “ (1 <= INT_MAX) ” 
+  &&  “ ((INT_MIN) <= 1) ”
+.
+
+Definition cycpattern_check_safety_wit_16 := 
+forall (b0: Z) (a0: Z) (b_l: (@list Z)) (a_l: (@list Z)) (hit: Z) (rotate: Z) (n: Z) (i: Z) (PreH1 : (0 <= ((string_length (b_l)) + 1 ))) (PreH2 : (0 <= ((string_length (a_l)) + 1 ))) (PreH3 : (hit <> 0)) (PreH4 : (rotate <> 0)) (PreH5 : ((n + 1 ) < INT_MAX)) (PreH6 : (valid_string a_l )) (PreH7 : (valid_string b_l )) (PreH8 : ((string_length (a_l)) < INT_MAX)) (PreH9 : (n = (string_length (b_l)))) (PreH10 : (rotation_success_154 a_l b_l i (rotate_at_154 (b_l) (i)) )) ,
+  (CharArray.full b0 ((string_length (b_l)) + 1 ) (c_string (b_l)) )
+  **  (CharArray.full a0 ((string_length (a_l)) + 1 ) (c_string (a_l)) )
+  **  ((( &( "hit" ) )) # Ptr  |-> hit)
+  **  ((( &( "rotate" ) )) # Ptr  |-> rotate)
+  **  ((( &( "n" ) )) # Int  |-> n)
+  **  ((( &( "a" ) )) # Ptr  |-> a0)
+  **  ((( &( "b" ) )) # Ptr  |-> b0)
+  **  ((( &( "i" ) )) # Int  |-> i)
+|--
+  “ (1 <= INT_MAX) ” 
+  &&  “ ((INT_MIN) <= 1) ”
+.
+
+Definition cycpattern_check_safety_wit_17 := 
+(
+forall (b0: Z) (a0: Z) (b_l: (@list Z)) (a_l: (@list Z)) (hit: Z) (rotate: Z) (n: Z) (i: Z) (PreH1 : (hit = 0)) (PreH2 : (rotate <> 0)) (PreH3 : ((n + 1 ) < INT_MAX)) (PreH4 : (valid_string a_l )) (PreH5 : (valid_string b_l )) (PreH6 : ((string_length (a_l)) < INT_MAX)) (PreH7 : (n = (string_length (b_l)))) (PreH8 : (rotation_scan_state_154 a_l b_l (i + 1 ) )) ,
+  ((( &( "hit" ) )) # Ptr  |-> hit)
+  **  ((( &( "rotate" ) )) # Ptr  |-> rotate)
+  **  ((( &( "n" ) )) # Int  |-> n)
+  **  ((( &( "a" ) )) # Ptr  |-> a0)
+  **  ((( &( "b" ) )) # Ptr  |-> b0)
+  **  ((( &( "i" ) )) # Int  |-> i)
+  **  (store_string a0 a_l )
+  **  (store_string b0 b_l )
+  **  (CharArray.undef_full rotate (n + 1 ) )
+|--
+  “ ((i + 1 ) <= INT_MAX) ” 
+  &&  “ ((INT_MIN) <= (i + 1 )) ”
+) \/
+(
+forall (b0: Z) (a0: Z) (b_l: (@list Z)) (a_l: (@list Z)) (hit: Z) (rotate: Z) (n: Z) (i: Z) (PreH1 : (hit = 0)) (PreH2 : (rotate <> 0)) (PreH3 : ((n + 1 ) < INT_MAX)) (PreH4 : (valid_string a_l )) (PreH5 : (valid_string b_l )) (PreH6 : ((string_length (a_l)) < INT_MAX)) (PreH7 : (n = (string_length (b_l)))) (PreH8 : (rotation_scan_state_154 a_l b_l (i + 1 ) )) ,
+  ((( &( "hit" ) )) # Ptr  |-> hit)
+  **  ((( &( "rotate" ) )) # Ptr  |-> rotate)
+  **  ((( &( "n" ) )) # Int  |-> n)
+  **  ((( &( "a" ) )) # Ptr  |-> a0)
+  **  ((( &( "b" ) )) # Ptr  |-> b0)
+  **  ((( &( "i" ) )) # Int  |-> i)
+  **  (store_string a0 a_l )
+  **  (store_string b0 b_l )
+  **  (CharArray.undef_full rotate (n + 1 ) )
+|--
+  “ ((i + 1 ) <= INT_MAX) ” 
+  &&  “ ((INT_MIN) <= (i + 1 )) ”
+).
+
+Definition cycpattern_check_safety_wit_17_split_goal_1 := 
+forall (b0: Z) (a0: Z) (b_l: (@list Z)) (a_l: (@list Z)) (hit: Z) (rotate: Z) (n: Z) (i: Z) (PreH1 : (hit = 0)) (PreH2 : (rotate <> 0)) (PreH3 : ((n + 1 ) < INT_MAX)) (PreH4 : (valid_string a_l )) (PreH5 : (valid_string b_l )) (PreH6 : ((string_length (a_l)) < INT_MAX)) (PreH7 : (n = (string_length (b_l)))) (PreH8 : (rotation_scan_state_154 a_l b_l (i + 1 ) )) ,
+  ((( &( "hit" ) )) # Ptr  |-> hit)
+  **  ((( &( "rotate" ) )) # Ptr  |-> rotate)
+  **  ((( &( "n" ) )) # Int  |-> n)
+  **  ((( &( "a" ) )) # Ptr  |-> a0)
+  **  ((( &( "b" ) )) # Ptr  |-> b0)
+  **  ((( &( "i" ) )) # Int  |-> i)
+  **  (store_string a0 a_l )
+  **  (store_string b0 b_l )
+  **  (CharArray.undef_full rotate (n + 1 ) )
+|--
+  “ ((i + 1 ) <= INT_MAX) ”
+.
+
+Definition cycpattern_check_safety_wit_17_split_goal_2 := 
+forall (b0: Z) (a0: Z) (b_l: (@list Z)) (a_l: (@list Z)) (hit: Z) (rotate: Z) (n: Z) (i: Z) (PreH1 : (hit = 0)) (PreH2 : (rotate <> 0)) (PreH3 : ((n + 1 ) < INT_MAX)) (PreH4 : (valid_string a_l )) (PreH5 : (valid_string b_l )) (PreH6 : ((string_length (a_l)) < INT_MAX)) (PreH7 : (n = (string_length (b_l)))) (PreH8 : (rotation_scan_state_154 a_l b_l (i + 1 ) )) ,
+  ((( &( "hit" ) )) # Ptr  |-> hit)
+  **  ((( &( "rotate" ) )) # Ptr  |-> rotate)
+  **  ((( &( "n" ) )) # Int  |-> n)
+  **  ((( &( "a" ) )) # Ptr  |-> a0)
+  **  ((( &( "b" ) )) # Ptr  |-> b0)
+  **  ((( &( "i" ) )) # Int  |-> i)
+  **  (store_string a0 a_l )
+  **  (store_string b0 b_l )
+  **  (CharArray.undef_full rotate (n + 1 ) )
+|--
+  “ ((INT_MIN) <= (i + 1 )) ”
+.
+
+Definition cycpattern_check_safety_wit_18 := 
+forall (b0: Z) (a0: Z) (b_l: (@list Z)) (a_l: (@list Z)) (rotate: Z) (n: Z) (i: Z) (PreH1 : (i >= n)) (PreH2 : (0 <= i)) (PreH3 : (i <= n)) (PreH4 : (rotate <> 0)) (PreH5 : ((n + 1 ) < INT_MAX)) (PreH6 : (valid_string a_l )) (PreH7 : (valid_string b_l )) (PreH8 : ((string_length (a_l)) < INT_MAX)) (PreH9 : (n = (string_length (b_l)))) (PreH10 : (rotation_scan_state_154 a_l b_l i )) ,
+  ((( &( "i" ) )) # Int  |-> i)
+  **  ((( &( "n" ) )) # Int  |-> n)
+  **  ((( &( "rotate" ) )) # Ptr  |-> rotate)
+  **  ((( &( "a" ) )) # Ptr  |-> a0)
+  **  ((( &( "b" ) )) # Ptr  |-> b0)
+  **  (store_string a0 a_l )
+  **  (store_string b0 b_l )
+  **  (CharArray.undef_full rotate (n + 1 ) )
+|--
+  “ ((n + 1 ) <= INT_MAX) ” 
+  &&  “ ((INT_MIN) <= (n + 1 )) ”
+.
+
+Definition cycpattern_check_safety_wit_19 := 
+forall (b0: Z) (a0: Z) (b_l: (@list Z)) (a_l: (@list Z)) (rotate: Z) (n: Z) (i: Z) (PreH1 : (i >= n)) (PreH2 : (0 <= i)) (PreH3 : (i <= n)) (PreH4 : (rotate <> 0)) (PreH5 : ((n + 1 ) < INT_MAX)) (PreH6 : (valid_string a_l )) (PreH7 : (valid_string b_l )) (PreH8 : ((string_length (a_l)) < INT_MAX)) (PreH9 : (n = (string_length (b_l)))) (PreH10 : (rotation_scan_state_154 a_l b_l i )) ,
+  ((( &( "i" ) )) # Int  |-> i)
+  **  ((( &( "n" ) )) # Int  |-> n)
+  **  ((( &( "rotate" ) )) # Ptr  |-> rotate)
+  **  ((( &( "a" ) )) # Ptr  |-> a0)
+  **  ((( &( "b" ) )) # Ptr  |-> b0)
+  **  (store_string a0 a_l )
+  **  (store_string b0 b_l )
+  **  (CharArray.undef_full rotate (n + 1 ) )
+|--
+  “ (1 <= INT_MAX) ” 
+  &&  “ ((INT_MIN) <= 1) ”
+.
+
+Definition cycpattern_check_safety_wit_20 := 
+forall (b0: Z) (a0: Z) (b_l: (@list Z)) (a_l: (@list Z)) (rotate: Z) (n: Z) (i: Z) (PreH1 : (0 <= ((string_length (b_l)) + 1 ))) (PreH2 : (0 <= ((string_length (a_l)) + 1 ))) (PreH3 : (i >= n)) (PreH4 : (0 <= i)) (PreH5 : (i <= n)) (PreH6 : (rotate <> 0)) (PreH7 : ((n + 1 ) < INT_MAX)) (PreH8 : (valid_string a_l )) (PreH9 : (valid_string b_l )) (PreH10 : ((string_length (a_l)) < INT_MAX)) (PreH11 : (n = (string_length (b_l)))) (PreH12 : (rotation_scan_state_154 a_l b_l i )) ,
+  (CharArray.full b0 ((string_length (b_l)) + 1 ) (c_string (b_l)) )
+  **  (CharArray.full a0 ((string_length (a_l)) + 1 ) (c_string (a_l)) )
+  **  ((( &( "i" ) )) # Int  |-> i)
+  **  ((( &( "n" ) )) # Int  |-> n)
+  **  ((( &( "rotate" ) )) # Ptr  |-> rotate)
+  **  ((( &( "a" ) )) # Ptr  |-> a0)
+  **  ((( &( "b" ) )) # Ptr  |-> b0)
+|--
+  “ (0 <= INT_MAX) ” 
+  &&  “ ((INT_MIN) <= 0) ”
+.
+
+Definition cycpattern_check_entail_wit_1 := 
+(
+forall (b_pre: Z) (a_pre: Z) (b0: Z) (a0: Z) (b_l: (@list Z)) (a_l: (@list Z)) (retval: Z) (retval_2: Z) (PreH1 : (retval_2 <> 0)) (PreH2 : (retval_2 <> 0)) (PreH3 : (retval = (string_length (b_l)))) (PreH4 : (0 <= ((string_length (b_l)) + 1 ))) (PreH5 : (0 <= ((string_length (a_l)) + 1 ))) (PreH6 : (a_pre = a0)) (PreH7 : (b_pre = b0)) (PreH8 : (problem_154_pre_z a_l b_l )) (PreH9 : (valid_string a_l )) (PreH10 : (valid_string b_l )) (PreH11 : ((string_length (a_l)) < INT_MAX)) (PreH12 : (((string_length (b_l)) + 1 ) < INT_MAX)) ,
+  (CharArray.undef_full retval_2 (retval + 1 ) )
+  **  (CharArray.full b_pre ((string_length (b_l)) + 1 ) (c_string (b_l)) )
+  **  (CharArray.full a0 ((string_length (a_l)) + 1 ) (c_string (a_l)) )
+  **  ((( &( "b" ) )) # Ptr  |-> b_pre)
+  **  ((( &( "a" ) )) # Ptr  |-> a_pre)
+|--
+  “ (0 <= 0) ” 
+  &&  “ (0 <= retval) ” 
+  &&  “ (retval_2 <> 0) ” 
+  &&  “ ((retval + 1 ) < INT_MAX) ” 
+  &&  “ (valid_string a_l ) ” 
+  &&  “ (valid_string b_l ) ” 
+  &&  “ ((string_length (a_l)) < INT_MAX) ” 
+  &&  “ (retval = (string_length (b_l))) ” 
+  &&  “ (rotation_scan_state_154 a_l b_l 0 ) ”
+  &&  ((( &( "a" ) )) # Ptr  |-> a0)
+  **  ((( &( "b" ) )) # Ptr  |-> b0)
+  **  (store_string a0 a_l )
+  **  (store_string b0 b_l )
+  **  (CharArray.undef_full retval_2 (retval + 1 ) )
+) \/
+(
+forall (b_pre: Z) (a_pre: Z) (b0: Z) (a0: Z) (b_l: (@list Z)) (a_l: (@list Z)) (retval: Z) (retval_2: Z) (PreH1 : (retval_2 <> 0)) (PreH2 : (retval_2 <> 0)) (PreH3 : (retval = (string_length (b_l)))) (PreH4 : (0 <= ((string_length (b_l)) + 1 ))) (PreH5 : (0 <= ((string_length (a_l)) + 1 ))) (PreH6 : (a_pre = a0)) (PreH7 : (b_pre = b0)) (PreH8 : (problem_154_pre_z a_l b_l )) (PreH9 : (valid_string a_l )) (PreH10 : (valid_string b_l )) (PreH11 : ((string_length (a_l)) < INT_MAX)) (PreH12 : (((string_length (b_l)) + 1 ) < INT_MAX)) ,
+  (CharArray.undef_full retval_2 (retval + 1 ) )
+  **  (CharArray.full b_pre ((string_length (b_l)) + 1 ) (c_string (b_l)) )
+|--
+  “ (rotation_scan_state_154 a_l b_l 0 ) ” 
+  &&  “ (0 <= retval) ”
+  &&  (CharArray.full b0 ((string_length (b_l)) + 1 ) (c_string (b_l)) )
+  **  (CharArray.undef_full retval_2 (retval + 1 ) )
+).
+
+Definition cycpattern_check_entail_wit_1_split_goal_1 := 
+forall (b_pre: Z) (a_pre: Z) (b0: Z) (a0: Z) (b_l: (@list Z)) (a_l: (@list Z)) (retval: Z) (retval_2: Z) (PreH1 : (retval_2 <> 0)) (PreH2 : (retval_2 <> 0)) (PreH3 : (retval = (string_length (b_l)))) (PreH4 : (0 <= ((string_length (b_l)) + 1 ))) (PreH5 : (0 <= ((string_length (a_l)) + 1 ))) (PreH6 : (a_pre = a0)) (PreH7 : (b_pre = b0)) (PreH8 : (problem_154_pre_z a_l b_l )) (PreH9 : (valid_string a_l )) (PreH10 : (valid_string b_l )) (PreH11 : ((string_length (a_l)) < INT_MAX)) (PreH12 : (((string_length (b_l)) + 1 ) < INT_MAX)) ,
+  (CharArray.undef_full retval_2 (retval + 1 ) )
+  **  (CharArray.full b_pre ((string_length (b_l)) + 1 ) (c_string (b_l)) )
+|--
+  “ (rotation_scan_state_154 a_l b_l 0 ) ”
+.
+
+Definition cycpattern_check_entail_wit_1_split_goal_2 := 
+forall (b_pre: Z) (a_pre: Z) (b0: Z) (a0: Z) (b_l: (@list Z)) (a_l: (@list Z)) (retval: Z) (retval_2: Z) (PreH1 : (retval_2 <> 0)) (PreH2 : (retval_2 <> 0)) (PreH3 : (retval = (string_length (b_l)))) (PreH4 : (0 <= ((string_length (b_l)) + 1 ))) (PreH5 : (0 <= ((string_length (a_l)) + 1 ))) (PreH6 : (a_pre = a0)) (PreH7 : (b_pre = b0)) (PreH8 : (problem_154_pre_z a_l b_l )) (PreH9 : (valid_string a_l )) (PreH10 : (valid_string b_l )) (PreH11 : ((string_length (a_l)) < INT_MAX)) (PreH12 : (((string_length (b_l)) + 1 ) < INT_MAX)) ,
+  (CharArray.undef_full retval_2 (retval + 1 ) )
+  **  (CharArray.full b_pre ((string_length (b_l)) + 1 ) (c_string (b_l)) )
+|--
+  “ (0 <= retval) ”
+.
+
+Definition cycpattern_check_entail_wit_1_split_goal_spatial := 
+forall (b_pre: Z) (a_pre: Z) (b0: Z) (a0: Z) (b_l: (@list Z)) (a_l: (@list Z)) (retval: Z) (retval_2: Z) (PreH1 : (retval_2 <> 0)) (PreH2 : (retval_2 <> 0)) (PreH3 : (retval = (string_length (b_l)))) (PreH4 : (0 <= ((string_length (b_l)) + 1 ))) (PreH5 : (0 <= ((string_length (a_l)) + 1 ))) (PreH6 : (a_pre = a0)) (PreH7 : (b_pre = b0)) (PreH8 : (problem_154_pre_z a_l b_l )) (PreH9 : (valid_string a_l )) (PreH10 : (valid_string b_l )) (PreH11 : ((string_length (a_l)) < INT_MAX)) (PreH12 : (((string_length (b_l)) + 1 ) < INT_MAX)) ,
+  (CharArray.undef_full retval_2 (retval + 1 ) )
+  **  (CharArray.full b_pre ((string_length (b_l)) + 1 ) (c_string (b_l)) )
+|--
+  (CharArray.full b0 ((string_length (b_l)) + 1 ) (c_string (b_l)) )
+  **  (CharArray.undef_full retval_2 (retval + 1 ) )
+.
+
+Definition cycpattern_check_entail_wit_2 := 
+(
+forall (b0: Z) (a0: Z) (b_l: (@list Z)) (a_l: (@list Z)) (rotate: Z) (n: Z) (i: Z) (PreH1 : (i < n)) (PreH2 : (0 <= i)) (PreH3 : (i <= n)) (PreH4 : (rotate <> 0)) (PreH5 : ((n + 1 ) < INT_MAX)) (PreH6 : (valid_string a_l )) (PreH7 : (valid_string b_l )) (PreH8 : ((string_length (a_l)) < INT_MAX)) (PreH9 : (n = (string_length (b_l)))) (PreH10 : (rotation_scan_state_154 a_l b_l i )) ,
+  (store_string a0 a_l )
+  **  (store_string b0 b_l )
+  **  (CharArray.undef_full rotate (n + 1 ) )
+|--
+  EX (rotate_l: (@list Z)) ,
+  “ (0 <= 0) ” 
+  &&  “ (0 <= n) ” 
+  &&  “ (0 < n) ” 
+  &&  “ (0 <= i) ” 
+  &&  “ (i < n) ” 
+  &&  “ (rotate <> 0) ” 
+  &&  “ ((n + 1 ) < INT_MAX) ” 
+  &&  “ (valid_string a_l ) ” 
+  &&  “ (valid_string b_l ) ” 
+  &&  “ ((string_length (a_l)) < INT_MAX) ” 
+  &&  “ (n = (string_length (b_l))) ” 
+  &&  “ (rotation_scan_state_154 a_l b_l i ) ” 
+  &&  “ (rotation_prefix_154 b_l i 0 rotate_l ) ”
+  &&  (store_string a0 a_l )
+  **  (store_string b0 b_l )
+  **  (CharArray.full rotate 0 rotate_l )
+  **  (CharArray.undef_seg rotate 0 (n + 1 ) )
+) \/
+(
+forall (b_l: (@list Z)) (a_l: (@list Z)) (rotate: Z) (n: Z) (i: Z) (PreH1 : (0 <= ((string_length (b_l)) + 1 ))) (PreH2 : (0 <= ((string_length (a_l)) + 1 ))) (PreH3 : (i < n)) (PreH4 : (0 <= i)) (PreH5 : (i <= n)) (PreH6 : (rotate <> 0)) (PreH7 : ((n + 1 ) < INT_MAX)) (PreH8 : (valid_string a_l )) (PreH9 : (valid_string b_l )) (PreH10 : ((string_length (a_l)) < INT_MAX)) (PreH11 : (n = (string_length (b_l)))) (PreH12 : (rotation_scan_state_154 a_l b_l i )) ,
+  (CharArray.undef_full rotate (n + 1 ) )
+|--
+  “ (rotation_prefix_154 b_l i 0 (@nil Z) ) ”
+  &&  (CharArray.undef_full rotate (n + 1 ) )
+).
+
+Definition cycpattern_check_entail_wit_2_split_goal_1 := 
+forall (b_l: (@list Z)) (a_l: (@list Z)) (rotate: Z) (n: Z) (i: Z) (PreH1 : (0 <= ((string_length (b_l)) + 1 ))) (PreH2 : (0 <= ((string_length (a_l)) + 1 ))) (PreH3 : (i < n)) (PreH4 : (0 <= i)) (PreH5 : (i <= n)) (PreH6 : (rotate <> 0)) (PreH7 : ((n + 1 ) < INT_MAX)) (PreH8 : (valid_string a_l )) (PreH9 : (valid_string b_l )) (PreH10 : ((string_length (a_l)) < INT_MAX)) (PreH11 : (n = (string_length (b_l)))) (PreH12 : (rotation_scan_state_154 a_l b_l i )) ,
+  (CharArray.undef_full rotate (n + 1 ) )
+|--
+  “ (rotation_prefix_154 b_l i 0 (@nil Z) ) ”
+.
+
+Definition cycpattern_check_entail_wit_2_split_goal_spatial := 
+forall (b_l: (@list Z)) (a_l: (@list Z)) (rotate: Z) (n: Z) (i: Z) (PreH1 : (0 <= ((string_length (b_l)) + 1 ))) (PreH2 : (0 <= ((string_length (a_l)) + 1 ))) (PreH3 : (i < n)) (PreH4 : (0 <= i)) (PreH5 : (i <= n)) (PreH6 : (rotate <> 0)) (PreH7 : ((n + 1 ) < INT_MAX)) (PreH8 : (valid_string a_l )) (PreH9 : (valid_string b_l )) (PreH10 : ((string_length (a_l)) < INT_MAX)) (PreH11 : (n = (string_length (b_l)))) (PreH12 : (rotation_scan_state_154 a_l b_l i )) ,
+  (CharArray.undef_full rotate (n + 1 ) )
+|--
+  (CharArray.undef_full rotate (n + 1 ) )
+.
+
+Definition cycpattern_check_entail_wit_3_1 := 
+(
+forall (b0: Z) (a0: Z) (b_l: (@list Z)) (a_l: (@list Z)) (rotate_l_2: (@list Z)) (rotate: Z) (i: Z) (n: Z) (j: Z) (PreH1 : (j < (n - i ))) (PreH2 : (j < n)) (PreH3 : (0 <= j)) (PreH4 : (j <= n)) (PreH5 : (0 < n)) (PreH6 : (0 <= i)) (PreH7 : (i < n)) (PreH8 : (rotate <> 0)) (PreH9 : ((n + 1 ) < INT_MAX)) (PreH10 : (valid_string a_l )) (PreH11 : (valid_string b_l )) (PreH12 : ((string_length (a_l)) < INT_MAX)) (PreH13 : (n = (string_length (b_l)))) (PreH14 : (rotation_scan_state_154 a_l b_l i )) (PreH15 : (rotation_prefix_154 b_l i j rotate_l_2 )) ,
+  (store_string a0 a_l )
+  **  (store_string b0 b_l )
+  **  (CharArray.full rotate j rotate_l_2 )
+  **  (CharArray.undef_seg rotate j (n + 1 ) )
+|--
+  EX (rotate_l: (@list Z)) ,
+  “ ((i + j ) = ((i + j ) % ( n ) )) ” 
+  &&  “ (0 <= (i + j )) ” 
+  &&  “ ((i + j ) < n) ” 
+  &&  “ (0 <= j) ” 
+  &&  “ (j < n) ” 
+  &&  “ (0 < n) ” 
+  &&  “ (0 <= i) ” 
+  &&  “ (i < n) ” 
+  &&  “ (rotate <> 0) ” 
+  &&  “ ((n + 1 ) < INT_MAX) ” 
+  &&  “ (valid_string a_l ) ” 
+  &&  “ (valid_string b_l ) ” 
+  &&  “ ((string_length (a_l)) < INT_MAX) ” 
+  &&  “ (n = (string_length (b_l))) ” 
+  &&  “ (rotation_scan_state_154 a_l b_l i ) ” 
+  &&  “ (rotation_prefix_154 b_l i j rotate_l ) ”
+  &&  (store_string a0 a_l )
+  **  (store_string b0 b_l )
+  **  (CharArray.full rotate j rotate_l )
+  **  (CharArray.undef_seg rotate j (n + 1 ) )
+) \/
+(
+forall (b_l: (@list Z)) (a_l: (@list Z)) (rotate_l_2: (@list Z)) (rotate: Z) (i: Z) (n: Z) (j: Z) (PreH1 : (0 <= ((string_length (b_l)) + 1 ))) (PreH2 : (0 <= ((string_length (a_l)) + 1 ))) (PreH3 : (j < (n - i ))) (PreH4 : (j < n)) (PreH5 : (0 <= j)) (PreH6 : (j <= n)) (PreH7 : (0 < n)) (PreH8 : (0 <= i)) (PreH9 : (i < n)) (PreH10 : (rotate <> 0)) (PreH11 : ((n + 1 ) < INT_MAX)) (PreH12 : (valid_string a_l )) (PreH13 : (valid_string b_l )) (PreH14 : ((string_length (a_l)) < INT_MAX)) (PreH15 : (n = (string_length (b_l)))) (PreH16 : (rotation_scan_state_154 a_l b_l i )) (PreH17 : (rotation_prefix_154 b_l i j rotate_l_2 )) ,
+  TT && emp 
+|--
+  “ ((i + j ) = ((i + j ) % ( n ) )) ”
+  &&  emp
+).
+
+Definition cycpattern_check_entail_wit_3_1_split_goal_1 := 
+forall (b_l: (@list Z)) (a_l: (@list Z)) (rotate_l_2: (@list Z)) (rotate: Z) (i: Z) (n: Z) (j: Z) (PreH1 : (0 <= ((string_length (b_l)) + 1 ))) (PreH2 : (0 <= ((string_length (a_l)) + 1 ))) (PreH3 : (j < (n - i ))) (PreH4 : (j < n)) (PreH5 : (0 <= j)) (PreH6 : (j <= n)) (PreH7 : (0 < n)) (PreH8 : (0 <= i)) (PreH9 : (i < n)) (PreH10 : (rotate <> 0)) (PreH11 : ((n + 1 ) < INT_MAX)) (PreH12 : (valid_string a_l )) (PreH13 : (valid_string b_l )) (PreH14 : ((string_length (a_l)) < INT_MAX)) (PreH15 : (n = (string_length (b_l)))) (PreH16 : (rotation_scan_state_154 a_l b_l i )) (PreH17 : (rotation_prefix_154 b_l i j rotate_l_2 )) ,
+  TT && emp 
+|--
+  “ ((i + j ) = ((i + j ) % ( n ) )) ”
+.
+
+Definition cycpattern_check_entail_wit_3_2 := 
+(
+forall (b0: Z) (a0: Z) (b_l: (@list Z)) (a_l: (@list Z)) (rotate_l_2: (@list Z)) (rotate: Z) (i: Z) (n: Z) (j: Z) (PreH1 : (j >= (n - i ))) (PreH2 : (j < n)) (PreH3 : (0 <= j)) (PreH4 : (j <= n)) (PreH5 : (0 < n)) (PreH6 : (0 <= i)) (PreH7 : (i < n)) (PreH8 : (rotate <> 0)) (PreH9 : ((n + 1 ) < INT_MAX)) (PreH10 : (valid_string a_l )) (PreH11 : (valid_string b_l )) (PreH12 : ((string_length (a_l)) < INT_MAX)) (PreH13 : (n = (string_length (b_l)))) (PreH14 : (rotation_scan_state_154 a_l b_l i )) (PreH15 : (rotation_prefix_154 b_l i j rotate_l_2 )) ,
+  (store_string a0 a_l )
+  **  (store_string b0 b_l )
+  **  (CharArray.full rotate j rotate_l_2 )
+  **  (CharArray.undef_seg rotate j (n + 1 ) )
+|--
+  EX (rotate_l: (@list Z)) ,
+  “ ((j - (n - i ) ) = ((i + j ) % ( n ) )) ” 
+  &&  “ (0 <= (j - (n - i ) )) ” 
+  &&  “ ((j - (n - i ) ) < n) ” 
+  &&  “ (0 <= j) ” 
+  &&  “ (j < n) ” 
+  &&  “ (0 < n) ” 
+  &&  “ (0 <= i) ” 
+  &&  “ (i < n) ” 
+  &&  “ (rotate <> 0) ” 
+  &&  “ ((n + 1 ) < INT_MAX) ” 
+  &&  “ (valid_string a_l ) ” 
+  &&  “ (valid_string b_l ) ” 
+  &&  “ ((string_length (a_l)) < INT_MAX) ” 
+  &&  “ (n = (string_length (b_l))) ” 
+  &&  “ (rotation_scan_state_154 a_l b_l i ) ” 
+  &&  “ (rotation_prefix_154 b_l i j rotate_l ) ”
+  &&  (store_string a0 a_l )
+  **  (store_string b0 b_l )
+  **  (CharArray.full rotate j rotate_l )
+  **  (CharArray.undef_seg rotate j (n + 1 ) )
+) \/
+(
+forall (b_l: (@list Z)) (a_l: (@list Z)) (rotate_l_2: (@list Z)) (rotate: Z) (i: Z) (n: Z) (j: Z) (PreH1 : (0 <= ((string_length (b_l)) + 1 ))) (PreH2 : (0 <= ((string_length (a_l)) + 1 ))) (PreH3 : (j >= (n - i ))) (PreH4 : (j < n)) (PreH5 : (0 <= j)) (PreH6 : (j <= n)) (PreH7 : (0 < n)) (PreH8 : (0 <= i)) (PreH9 : (i < n)) (PreH10 : (rotate <> 0)) (PreH11 : ((n + 1 ) < INT_MAX)) (PreH12 : (valid_string a_l )) (PreH13 : (valid_string b_l )) (PreH14 : ((string_length (a_l)) < INT_MAX)) (PreH15 : (n = (string_length (b_l)))) (PreH16 : (rotation_scan_state_154 a_l b_l i )) (PreH17 : (rotation_prefix_154 b_l i j rotate_l_2 )) ,
+  TT && emp 
+|--
+  “ ((j - (n - i ) ) = ((i + j ) % ( n ) )) ”
+  &&  emp
+).
+
+Definition cycpattern_check_entail_wit_3_2_split_goal_1 := 
+forall (b_l: (@list Z)) (a_l: (@list Z)) (rotate_l_2: (@list Z)) (rotate: Z) (i: Z) (n: Z) (j: Z) (PreH1 : (0 <= ((string_length (b_l)) + 1 ))) (PreH2 : (0 <= ((string_length (a_l)) + 1 ))) (PreH3 : (j >= (n - i ))) (PreH4 : (j < n)) (PreH5 : (0 <= j)) (PreH6 : (j <= n)) (PreH7 : (0 < n)) (PreH8 : (0 <= i)) (PreH9 : (i < n)) (PreH10 : (rotate <> 0)) (PreH11 : ((n + 1 ) < INT_MAX)) (PreH12 : (valid_string a_l )) (PreH13 : (valid_string b_l )) (PreH14 : ((string_length (a_l)) < INT_MAX)) (PreH15 : (n = (string_length (b_l)))) (PreH16 : (rotation_scan_state_154 a_l b_l i )) (PreH17 : (rotation_prefix_154 b_l i j rotate_l_2 )) ,
+  TT && emp 
+|--
+  “ ((j - (n - i ) ) = ((i + j ) % ( n ) )) ”
+.
+
+Definition cycpattern_check_entail_wit_4 := 
+(
+forall (b0: Z) (a0: Z) (b_l: (@list Z)) (a_l: (@list Z)) (rotate_l_2: (@list Z)) (idx: Z) (i: Z) (j: Z) (n: Z) (rotate: Z) (PreH1 : (idx = ((i + j ) % ( n ) ))) (PreH2 : (0 <= idx)) (PreH3 : (idx < n)) (PreH4 : (0 <= j)) (PreH5 : (j < n)) (PreH6 : (0 < n)) (PreH7 : (0 <= i)) (PreH8 : (i < n)) (PreH9 : (rotate <> 0)) (PreH10 : ((n + 1 ) < INT_MAX)) (PreH11 : (valid_string a_l )) (PreH12 : (valid_string b_l )) (PreH13 : ((string_length (a_l)) < INT_MAX)) (PreH14 : (n = (string_length (b_l)))) (PreH15 : (rotation_scan_state_154 a_l b_l i )) (PreH16 : (rotation_prefix_154 b_l i j rotate_l_2 )) ,
+  (store_string a0 a_l )
+  **  (store_string b0 b_l )
+  **  (CharArray.full rotate j rotate_l_2 )
+  **  (CharArray.undef_seg rotate j (n + 1 ) )
+|--
+  EX (rotate_l: (@list Z)) ,
+  “ ((Znth idx (c_string (b_l)) 0) = (Znth (idx) (b_l) (0))) ” 
+  &&  “ (idx = ((i + j ) % ( n ) )) ” 
+  &&  “ (0 <= (Znth idx (c_string (b_l)) 0)) ” 
+  &&  “ ((Znth idx (c_string (b_l)) 0) <= 127) ” 
+  &&  “ (0 <= idx) ” 
+  &&  “ (idx < n) ” 
+  &&  “ (0 <= j) ” 
+  &&  “ (j < n) ” 
+  &&  “ (0 < n) ” 
+  &&  “ (0 <= i) ” 
+  &&  “ (i < n) ” 
+  &&  “ (rotate <> 0) ” 
+  &&  “ ((n + 1 ) < INT_MAX) ” 
+  &&  “ (valid_string a_l ) ” 
+  &&  “ (valid_string b_l ) ” 
+  &&  “ ((string_length (a_l)) < INT_MAX) ” 
+  &&  “ (n = (string_length (b_l))) ” 
+  &&  “ (rotation_scan_state_154 a_l b_l i ) ” 
+  &&  “ (rotation_prefix_154 b_l i j rotate_l ) ”
+  &&  (store_string a0 a_l )
+  **  (store_string b0 b_l )
+  **  (CharArray.full rotate j rotate_l )
+  **  (CharArray.undef_seg rotate j (n + 1 ) )
+) \/
+(
+forall (b_l: (@list Z)) (a_l: (@list Z)) (rotate_l_2: (@list Z)) (idx: Z) (i: Z) (j: Z) (n: Z) (rotate: Z) (PreH1 : (0 <= ((string_length (b_l)) + 1 ))) (PreH2 : (0 <= ((string_length (a_l)) + 1 ))) (PreH3 : (idx = ((i + j ) % ( n ) ))) (PreH4 : (0 <= idx)) (PreH5 : (idx < n)) (PreH6 : (0 <= j)) (PreH7 : (j < n)) (PreH8 : (0 < n)) (PreH9 : (0 <= i)) (PreH10 : (i < n)) (PreH11 : (rotate <> 0)) (PreH12 : ((n + 1 ) < INT_MAX)) (PreH13 : (valid_string a_l )) (PreH14 : (valid_string b_l )) (PreH15 : ((string_length (a_l)) < INT_MAX)) (PreH16 : (n = (string_length (b_l)))) (PreH17 : (rotation_scan_state_154 a_l b_l i )) (PreH18 : (rotation_prefix_154 b_l i j rotate_l_2 )) ,
+  TT && emp 
+|--
+  “ ((Znth idx (c_string (b_l)) 0) <= 127) ” 
+  &&  “ (0 <= (Znth idx (c_string (b_l)) 0)) ” 
+  &&  “ ((Znth idx (c_string (b_l)) 0) = (Znth (idx) (b_l) (0))) ”
+  &&  emp
+).
+
+Definition cycpattern_check_entail_wit_4_split_goal_1 := 
+forall (b_l: (@list Z)) (a_l: (@list Z)) (rotate_l_2: (@list Z)) (idx: Z) (i: Z) (j: Z) (n: Z) (rotate: Z) (PreH1 : (0 <= ((string_length (b_l)) + 1 ))) (PreH2 : (0 <= ((string_length (a_l)) + 1 ))) (PreH3 : (idx = ((i + j ) % ( n ) ))) (PreH4 : (0 <= idx)) (PreH5 : (idx < n)) (PreH6 : (0 <= j)) (PreH7 : (j < n)) (PreH8 : (0 < n)) (PreH9 : (0 <= i)) (PreH10 : (i < n)) (PreH11 : (rotate <> 0)) (PreH12 : ((n + 1 ) < INT_MAX)) (PreH13 : (valid_string a_l )) (PreH14 : (valid_string b_l )) (PreH15 : ((string_length (a_l)) < INT_MAX)) (PreH16 : (n = (string_length (b_l)))) (PreH17 : (rotation_scan_state_154 a_l b_l i )) (PreH18 : (rotation_prefix_154 b_l i j rotate_l_2 )) ,
+  TT && emp 
+|--
+  “ ((Znth idx (c_string (b_l)) 0) <= 127) ”
+.
+
+Definition cycpattern_check_entail_wit_4_split_goal_2 := 
+forall (b_l: (@list Z)) (a_l: (@list Z)) (rotate_l_2: (@list Z)) (idx: Z) (i: Z) (j: Z) (n: Z) (rotate: Z) (PreH1 : (0 <= ((string_length (b_l)) + 1 ))) (PreH2 : (0 <= ((string_length (a_l)) + 1 ))) (PreH3 : (idx = ((i + j ) % ( n ) ))) (PreH4 : (0 <= idx)) (PreH5 : (idx < n)) (PreH6 : (0 <= j)) (PreH7 : (j < n)) (PreH8 : (0 < n)) (PreH9 : (0 <= i)) (PreH10 : (i < n)) (PreH11 : (rotate <> 0)) (PreH12 : ((n + 1 ) < INT_MAX)) (PreH13 : (valid_string a_l )) (PreH14 : (valid_string b_l )) (PreH15 : ((string_length (a_l)) < INT_MAX)) (PreH16 : (n = (string_length (b_l)))) (PreH17 : (rotation_scan_state_154 a_l b_l i )) (PreH18 : (rotation_prefix_154 b_l i j rotate_l_2 )) ,
+  TT && emp 
+|--
+  “ (0 <= (Znth idx (c_string (b_l)) 0)) ”
+.
+
+Definition cycpattern_check_entail_wit_4_split_goal_3 := 
+forall (b_l: (@list Z)) (a_l: (@list Z)) (rotate_l_2: (@list Z)) (idx: Z) (i: Z) (j: Z) (n: Z) (rotate: Z) (PreH1 : (0 <= ((string_length (b_l)) + 1 ))) (PreH2 : (0 <= ((string_length (a_l)) + 1 ))) (PreH3 : (idx = ((i + j ) % ( n ) ))) (PreH4 : (0 <= idx)) (PreH5 : (idx < n)) (PreH6 : (0 <= j)) (PreH7 : (j < n)) (PreH8 : (0 < n)) (PreH9 : (0 <= i)) (PreH10 : (i < n)) (PreH11 : (rotate <> 0)) (PreH12 : ((n + 1 ) < INT_MAX)) (PreH13 : (valid_string a_l )) (PreH14 : (valid_string b_l )) (PreH15 : ((string_length (a_l)) < INT_MAX)) (PreH16 : (n = (string_length (b_l)))) (PreH17 : (rotation_scan_state_154 a_l b_l i )) (PreH18 : (rotation_prefix_154 b_l i j rotate_l_2 )) ,
+  TT && emp 
+|--
+  “ ((Znth idx (c_string (b_l)) 0) = (Znth (idx) (b_l) (0))) ”
+.
+
+Definition cycpattern_check_entail_wit_5 := 
+(
+forall (b0: Z) (a0: Z) (b_l: (@list Z)) (a_l: (@list Z)) (rotate_l_2: (@list Z)) (ch: Z) (idx: Z) (i: Z) (j: Z) (n: Z) (rotate: Z) (PreH1 : (0 <= ((string_length (b_l)) + 1 ))) (PreH2 : (0 <= ((string_length (a_l)) + 1 ))) (PreH3 : (ch = (Znth (idx) (b_l) (0)))) (PreH4 : (idx = ((i + j ) % ( n ) ))) (PreH5 : (0 <= ch)) (PreH6 : (ch <= 127)) (PreH7 : (0 <= idx)) (PreH8 : (idx < n)) (PreH9 : (0 <= j)) (PreH10 : (j < n)) (PreH11 : (0 < n)) (PreH12 : (0 <= i)) (PreH13 : (i < n)) (PreH14 : (rotate <> 0)) (PreH15 : ((n + 1 ) < INT_MAX)) (PreH16 : (valid_string a_l )) (PreH17 : (valid_string b_l )) (PreH18 : ((string_length (a_l)) < INT_MAX)) (PreH19 : (n = (string_length (b_l)))) (PreH20 : (rotation_scan_state_154 a_l b_l i )) (PreH21 : (rotation_prefix_154 b_l i j rotate_l_2 )) ,
+  (CharArray.full rotate (j + 1 ) (app (rotate_l_2) ((cons (ch) ((@nil Z))))) )
+  **  (CharArray.undef_seg rotate (j + 1 ) (n + 1 ) )
+  **  (CharArray.full b0 ((string_length (b_l)) + 1 ) (c_string (b_l)) )
+  **  (CharArray.full a0 ((string_length (a_l)) + 1 ) (c_string (a_l)) )
+|--
+  EX (rotate_l: (@list Z)) ,
+  “ (0 <= (j + 1 )) ” 
+  &&  “ ((j + 1 ) <= n) ” 
+  &&  “ (0 < n) ” 
+  &&  “ (0 <= i) ” 
+  &&  “ (i < n) ” 
+  &&  “ (rotate <> 0) ” 
+  &&  “ ((n + 1 ) < INT_MAX) ” 
+  &&  “ (valid_string a_l ) ” 
+  &&  “ (valid_string b_l ) ” 
+  &&  “ ((string_length (a_l)) < INT_MAX) ” 
+  &&  “ (n = (string_length (b_l))) ” 
+  &&  “ (rotation_scan_state_154 a_l b_l i ) ” 
+  &&  “ (rotation_prefix_154 b_l i (j + 1 ) rotate_l ) ”
+  &&  (store_string a0 a_l )
+  **  (store_string b0 b_l )
+  **  (CharArray.full rotate (j + 1 ) rotate_l )
+  **  (CharArray.undef_seg rotate (j + 1 ) (n + 1 ) )
+) \/
+(
+forall (b_l: (@list Z)) (a_l: (@list Z)) (rotate_l_2: (@list Z)) (ch: Z) (idx: Z) (i: Z) (j: Z) (n: Z) (rotate: Z) (PreH1 : (0 <= ((string_length (b_l)) + 1 ))) (PreH2 : (0 <= ((string_length (a_l)) + 1 ))) (PreH3 : (ch = (Znth (idx) (b_l) (0)))) (PreH4 : (idx = ((i + j ) % ( n ) ))) (PreH5 : (0 <= ch)) (PreH6 : (ch <= 127)) (PreH7 : (0 <= idx)) (PreH8 : (idx < n)) (PreH9 : (0 <= j)) (PreH10 : (j < n)) (PreH11 : (0 < n)) (PreH12 : (0 <= i)) (PreH13 : (i < n)) (PreH14 : (rotate <> 0)) (PreH15 : ((n + 1 ) < INT_MAX)) (PreH16 : (valid_string a_l )) (PreH17 : (valid_string b_l )) (PreH18 : ((string_length (a_l)) < INT_MAX)) (PreH19 : (n = (string_length (b_l)))) (PreH20 : (rotation_scan_state_154 a_l b_l i )) (PreH21 : (rotation_prefix_154 b_l i j rotate_l_2 )) ,
+  TT && emp 
+|--
+  “ (rotation_prefix_154 b_l i (j + 1 ) (app (rotate_l_2) ((cons (ch) ((@nil Z))))) ) ”
+  &&  emp
+).
+
+Definition cycpattern_check_entail_wit_5_split_goal_1 := 
+forall (b_l: (@list Z)) (a_l: (@list Z)) (rotate_l_2: (@list Z)) (ch: Z) (idx: Z) (i: Z) (j: Z) (n: Z) (rotate: Z) (PreH1 : (0 <= ((string_length (b_l)) + 1 ))) (PreH2 : (0 <= ((string_length (a_l)) + 1 ))) (PreH3 : (ch = (Znth (idx) (b_l) (0)))) (PreH4 : (idx = ((i + j ) % ( n ) ))) (PreH5 : (0 <= ch)) (PreH6 : (ch <= 127)) (PreH7 : (0 <= idx)) (PreH8 : (idx < n)) (PreH9 : (0 <= j)) (PreH10 : (j < n)) (PreH11 : (0 < n)) (PreH12 : (0 <= i)) (PreH13 : (i < n)) (PreH14 : (rotate <> 0)) (PreH15 : ((n + 1 ) < INT_MAX)) (PreH16 : (valid_string a_l )) (PreH17 : (valid_string b_l )) (PreH18 : ((string_length (a_l)) < INT_MAX)) (PreH19 : (n = (string_length (b_l)))) (PreH20 : (rotation_scan_state_154 a_l b_l i )) (PreH21 : (rotation_prefix_154 b_l i j rotate_l_2 )) ,
+  TT && emp 
+|--
+  “ (rotation_prefix_154 b_l i (j + 1 ) (app (rotate_l_2) ((cons (ch) ((@nil Z))))) ) ”
+.
+
+Definition cycpattern_check_entail_wit_6 := 
+(
+forall (b0: Z) (a0: Z) (b_l: (@list Z)) (a_l: (@list Z)) (rotate_l: (@list Z)) (rotate: Z) (i: Z) (n: Z) (j: Z) (PreH1 : (0 <= ((string_length (b_l)) + 1 ))) (PreH2 : (0 <= ((string_length (a_l)) + 1 ))) (PreH3 : (j >= n)) (PreH4 : (0 <= j)) (PreH5 : (j <= n)) (PreH6 : (0 < n)) (PreH7 : (0 <= i)) (PreH8 : (i < n)) (PreH9 : (rotate <> 0)) (PreH10 : ((n + 1 ) < INT_MAX)) (PreH11 : (valid_string a_l )) (PreH12 : (valid_string b_l )) (PreH13 : ((string_length (a_l)) < INT_MAX)) (PreH14 : (n = (string_length (b_l)))) (PreH15 : (rotation_scan_state_154 a_l b_l i )) (PreH16 : (rotation_prefix_154 b_l i j rotate_l )) ,
+  (CharArray.full rotate (j + 1 ) (app (rotate_l) ((cons (0) ((@nil Z))))) )
+  **  (CharArray.undef_seg rotate (n + 1 ) (n + 1 ) )
+  **  (CharArray.full b0 ((string_length (b_l)) + 1 ) (c_string (b_l)) )
+  **  (CharArray.full a0 ((string_length (a_l)) + 1 ) (c_string (a_l)) )
+|--
+  “ (rotate <> 0) ” 
+  &&  “ ((n + 1 ) < INT_MAX) ” 
+  &&  “ (valid_string a_l ) ” 
+  &&  “ (valid_string b_l ) ” 
+  &&  “ ((string_length (a_l)) < INT_MAX) ” 
+  &&  “ (n = (string_length (b_l))) ” 
+  &&  “ (rotation_scan_state_154 a_l b_l i ) ” 
+  &&  “ (rotation_prefix_154 b_l i n (rotate_at_154 (b_l) (i)) ) ” 
+  &&  “ (valid_string (rotate_at_154 (b_l) (i)) ) ”
+  &&  (store_string a0 a_l )
+  **  (store_string b0 b_l )
+  **  (store_string rotate (rotate_at_154 (b_l) (i)) )
+) \/
+(
+forall (b_l: (@list Z)) (a_l: (@list Z)) (rotate_l: (@list Z)) (rotate: Z) (i: Z) (n: Z) (j: Z) (PreH1 : (0 <= (j + 1 ))) (PreH2 : (0 <= ((string_length (b_l)) + 1 ))) (PreH3 : (0 <= ((string_length (a_l)) + 1 ))) (PreH4 : (j >= n)) (PreH5 : (0 <= j)) (PreH6 : (j <= n)) (PreH7 : (0 < n)) (PreH8 : (0 <= i)) (PreH9 : (i < n)) (PreH10 : (rotate <> 0)) (PreH11 : ((n + 1 ) < INT_MAX)) (PreH12 : (valid_string a_l )) (PreH13 : (valid_string b_l )) (PreH14 : ((string_length (a_l)) < INT_MAX)) (PreH15 : (n = (string_length (b_l)))) (PreH16 : (rotation_scan_state_154 a_l b_l i )) (PreH17 : (rotation_prefix_154 b_l i j rotate_l )) ,
+  (CharArray.full rotate (j + 1 ) (app (rotate_l) ((cons (0) ((@nil Z))))) )
+|--
+  “ (valid_string (rotate_at_154 (b_l) (i)) ) ” 
+  &&  “ (rotation_prefix_154 b_l i n (rotate_at_154 (b_l) (i)) ) ”
+  &&  (CharArray.full rotate ((string_length ((rotate_at_154 (b_l) (i)))) + 1 ) (c_string ((rotate_at_154 (b_l) (i)))) )
+).
+
+Definition cycpattern_check_entail_wit_6_split_goal_1 := 
+forall (b_l: (@list Z)) (a_l: (@list Z)) (rotate_l: (@list Z)) (rotate: Z) (i: Z) (n: Z) (j: Z) (PreH1 : (0 <= (j + 1 ))) (PreH2 : (0 <= ((string_length (b_l)) + 1 ))) (PreH3 : (0 <= ((string_length (a_l)) + 1 ))) (PreH4 : (j >= n)) (PreH5 : (0 <= j)) (PreH6 : (j <= n)) (PreH7 : (0 < n)) (PreH8 : (0 <= i)) (PreH9 : (i < n)) (PreH10 : (rotate <> 0)) (PreH11 : ((n + 1 ) < INT_MAX)) (PreH12 : (valid_string a_l )) (PreH13 : (valid_string b_l )) (PreH14 : ((string_length (a_l)) < INT_MAX)) (PreH15 : (n = (string_length (b_l)))) (PreH16 : (rotation_scan_state_154 a_l b_l i )) (PreH17 : (rotation_prefix_154 b_l i j rotate_l )) ,
+  (CharArray.full rotate (j + 1 ) (app (rotate_l) ((cons (0) ((@nil Z))))) )
+|--
+  “ (valid_string (rotate_at_154 (b_l) (i)) ) ”
+.
+
+Definition cycpattern_check_entail_wit_6_split_goal_2 := 
+forall (b_l: (@list Z)) (a_l: (@list Z)) (rotate_l: (@list Z)) (rotate: Z) (i: Z) (n: Z) (j: Z) (PreH1 : (0 <= (j + 1 ))) (PreH2 : (0 <= ((string_length (b_l)) + 1 ))) (PreH3 : (0 <= ((string_length (a_l)) + 1 ))) (PreH4 : (j >= n)) (PreH5 : (0 <= j)) (PreH6 : (j <= n)) (PreH7 : (0 < n)) (PreH8 : (0 <= i)) (PreH9 : (i < n)) (PreH10 : (rotate <> 0)) (PreH11 : ((n + 1 ) < INT_MAX)) (PreH12 : (valid_string a_l )) (PreH13 : (valid_string b_l )) (PreH14 : ((string_length (a_l)) < INT_MAX)) (PreH15 : (n = (string_length (b_l)))) (PreH16 : (rotation_scan_state_154 a_l b_l i )) (PreH17 : (rotation_prefix_154 b_l i j rotate_l )) ,
+  (CharArray.full rotate (j + 1 ) (app (rotate_l) ((cons (0) ((@nil Z))))) )
+|--
+  “ (rotation_prefix_154 b_l i n (rotate_at_154 (b_l) (i)) ) ”
+.
+
+Definition cycpattern_check_entail_wit_6_split_goal_spatial := 
+forall (b_l: (@list Z)) (a_l: (@list Z)) (rotate_l: (@list Z)) (rotate: Z) (i: Z) (n: Z) (j: Z) (PreH1 : (0 <= (j + 1 ))) (PreH2 : (0 <= ((string_length (b_l)) + 1 ))) (PreH3 : (0 <= ((string_length (a_l)) + 1 ))) (PreH4 : (j >= n)) (PreH5 : (0 <= j)) (PreH6 : (j <= n)) (PreH7 : (0 < n)) (PreH8 : (0 <= i)) (PreH9 : (i < n)) (PreH10 : (rotate <> 0)) (PreH11 : ((n + 1 ) < INT_MAX)) (PreH12 : (valid_string a_l )) (PreH13 : (valid_string b_l )) (PreH14 : ((string_length (a_l)) < INT_MAX)) (PreH15 : (n = (string_length (b_l)))) (PreH16 : (rotation_scan_state_154 a_l b_l i )) (PreH17 : (rotation_prefix_154 b_l i j rotate_l )) ,
+  (CharArray.full rotate (j + 1 ) (app (rotate_l) ((cons (0) ((@nil Z))))) )
+|--
+  (CharArray.full rotate ((string_length ((rotate_at_154 (b_l) (i)))) + 1 ) (c_string ((rotate_at_154 (b_l) (i)))) )
+.
+
+Definition cycpattern_check_entail_wit_7 := 
+(
+forall (b0: Z) (a0: Z) (b_l: (@list Z)) (a_l: (@list Z)) (rotate: Z) (n: Z) (i: Z) (retval: Z) (PreH1 : (retval <> 0)) (PreH2 : (strstr_result a_l (rotate_at_154 (b_l) (i)) retval a0 )) (PreH3 : (0 <= ((string_length ((rotate_at_154 (b_l) (i)))) + 1 ))) (PreH4 : (0 <= ((string_length (b_l)) + 1 ))) (PreH5 : (0 <= ((string_length (a_l)) + 1 ))) (PreH6 : (rotate <> 0)) (PreH7 : ((n + 1 ) < INT_MAX)) (PreH8 : (valid_string a_l )) (PreH9 : (valid_string b_l )) (PreH10 : ((string_length (a_l)) < INT_MAX)) (PreH11 : (n = (string_length (b_l)))) (PreH12 : (rotation_scan_state_154 a_l b_l i )) (PreH13 : (rotation_prefix_154 b_l i n (rotate_at_154 (b_l) (i)) )) (PreH14 : (valid_string (rotate_at_154 (b_l) (i)) )) ,
+  (store_string a0 a_l )
+  **  (store_string rotate (rotate_at_154 (b_l) (i)) )
+  **  (CharArray.full b0 ((string_length (b_l)) + 1 ) (c_string (b_l)) )
+|--
+  “ (retval <> 0) ” 
+  &&  “ (rotate <> 0) ” 
+  &&  “ ((n + 1 ) < INT_MAX) ” 
+  &&  “ (valid_string a_l ) ” 
+  &&  “ (valid_string b_l ) ” 
+  &&  “ ((string_length (a_l)) < INT_MAX) ” 
+  &&  “ (n = (string_length (b_l))) ” 
+  &&  “ (rotation_success_154 a_l b_l i (rotate_at_154 (b_l) (i)) ) ”
+  &&  (store_string a0 a_l )
+  **  (store_string b0 b_l )
+  **  (CharArray.undef_full rotate (n + 1 ) )
+) \/
+(
+forall (a0: Z) (b_l: (@list Z)) (a_l: (@list Z)) (rotate: Z) (n: Z) (i: Z) (retval: Z) (PreH1 : (retval <> 0)) (PreH2 : (strstr_result a_l (rotate_at_154 (b_l) (i)) retval a0 )) (PreH3 : (0 <= ((string_length ((rotate_at_154 (b_l) (i)))) + 1 ))) (PreH4 : (0 <= ((string_length (b_l)) + 1 ))) (PreH5 : (0 <= ((string_length (a_l)) + 1 ))) (PreH6 : (rotate <> 0)) (PreH7 : ((n + 1 ) < INT_MAX)) (PreH8 : (valid_string a_l )) (PreH9 : (valid_string b_l )) (PreH10 : ((string_length (a_l)) < INT_MAX)) (PreH11 : (n = (string_length (b_l)))) (PreH12 : (rotation_scan_state_154 a_l b_l i )) (PreH13 : (rotation_prefix_154 b_l i n (rotate_at_154 (b_l) (i)) )) (PreH14 : (valid_string (rotate_at_154 (b_l) (i)) )) ,
+  (CharArray.full rotate ((string_length ((rotate_at_154 (b_l) (i)))) + 1 ) (c_string ((rotate_at_154 (b_l) (i)))) )
+|--
+  “ (rotation_success_154 a_l b_l i (rotate_at_154 (b_l) (i)) ) ”
+  &&  (CharArray.undef_full rotate (n + 1 ) )
+).
+
+Definition cycpattern_check_entail_wit_7_split_goal_1 := 
+forall (a0: Z) (b_l: (@list Z)) (a_l: (@list Z)) (rotate: Z) (n: Z) (i: Z) (retval: Z) (PreH1 : (retval <> 0)) (PreH2 : (strstr_result a_l (rotate_at_154 (b_l) (i)) retval a0 )) (PreH3 : (0 <= ((string_length ((rotate_at_154 (b_l) (i)))) + 1 ))) (PreH4 : (0 <= ((string_length (b_l)) + 1 ))) (PreH5 : (0 <= ((string_length (a_l)) + 1 ))) (PreH6 : (rotate <> 0)) (PreH7 : ((n + 1 ) < INT_MAX)) (PreH8 : (valid_string a_l )) (PreH9 : (valid_string b_l )) (PreH10 : ((string_length (a_l)) < INT_MAX)) (PreH11 : (n = (string_length (b_l)))) (PreH12 : (rotation_scan_state_154 a_l b_l i )) (PreH13 : (rotation_prefix_154 b_l i n (rotate_at_154 (b_l) (i)) )) (PreH14 : (valid_string (rotate_at_154 (b_l) (i)) )) ,
+  (CharArray.full rotate ((string_length ((rotate_at_154 (b_l) (i)))) + 1 ) (c_string ((rotate_at_154 (b_l) (i)))) )
+|--
+  “ (rotation_success_154 a_l b_l i (rotate_at_154 (b_l) (i)) ) ”
+.
+
+Definition cycpattern_check_entail_wit_7_split_goal_spatial := 
+forall (a0: Z) (b_l: (@list Z)) (a_l: (@list Z)) (rotate: Z) (n: Z) (i: Z) (retval: Z) (PreH1 : (retval <> 0)) (PreH2 : (strstr_result a_l (rotate_at_154 (b_l) (i)) retval a0 )) (PreH3 : (0 <= ((string_length ((rotate_at_154 (b_l) (i)))) + 1 ))) (PreH4 : (0 <= ((string_length (b_l)) + 1 ))) (PreH5 : (0 <= ((string_length (a_l)) + 1 ))) (PreH6 : (rotate <> 0)) (PreH7 : ((n + 1 ) < INT_MAX)) (PreH8 : (valid_string a_l )) (PreH9 : (valid_string b_l )) (PreH10 : ((string_length (a_l)) < INT_MAX)) (PreH11 : (n = (string_length (b_l)))) (PreH12 : (rotation_scan_state_154 a_l b_l i )) (PreH13 : (rotation_prefix_154 b_l i n (rotate_at_154 (b_l) (i)) )) (PreH14 : (valid_string (rotate_at_154 (b_l) (i)) )) ,
+  (CharArray.full rotate ((string_length ((rotate_at_154 (b_l) (i)))) + 1 ) (c_string ((rotate_at_154 (b_l) (i)))) )
+|--
+  (CharArray.undef_full rotate (n + 1 ) )
+.
+
+Definition cycpattern_check_entail_wit_8 := 
+(
+forall (b0: Z) (a0: Z) (b_l: (@list Z)) (a_l: (@list Z)) (rotate: Z) (n: Z) (i: Z) (retval: Z) (PreH1 : (retval = 0)) (PreH2 : (strstr_result a_l (rotate_at_154 (b_l) (i)) retval a0 )) (PreH3 : (0 <= ((string_length ((rotate_at_154 (b_l) (i)))) + 1 ))) (PreH4 : (0 <= ((string_length (b_l)) + 1 ))) (PreH5 : (0 <= ((string_length (a_l)) + 1 ))) (PreH6 : (rotate <> 0)) (PreH7 : ((n + 1 ) < INT_MAX)) (PreH8 : (valid_string a_l )) (PreH9 : (valid_string b_l )) (PreH10 : ((string_length (a_l)) < INT_MAX)) (PreH11 : (n = (string_length (b_l)))) (PreH12 : (rotation_scan_state_154 a_l b_l i )) (PreH13 : (rotation_prefix_154 b_l i n (rotate_at_154 (b_l) (i)) )) (PreH14 : (valid_string (rotate_at_154 (b_l) (i)) )) ,
+  (store_string a0 a_l )
+  **  (store_string rotate (rotate_at_154 (b_l) (i)) )
+  **  (CharArray.full b0 ((string_length (b_l)) + 1 ) (c_string (b_l)) )
+|--
+  “ (retval = 0) ” 
+  &&  “ (rotate <> 0) ” 
+  &&  “ ((n + 1 ) < INT_MAX) ” 
+  &&  “ (valid_string a_l ) ” 
+  &&  “ (valid_string b_l ) ” 
+  &&  “ ((string_length (a_l)) < INT_MAX) ” 
+  &&  “ (n = (string_length (b_l))) ” 
+  &&  “ (rotation_scan_state_154 a_l b_l (i + 1 ) ) ”
+  &&  (store_string a0 a_l )
+  **  (store_string b0 b_l )
+  **  (CharArray.undef_full rotate (n + 1 ) )
+) \/
+(
+forall (a0: Z) (b_l: (@list Z)) (a_l: (@list Z)) (rotate: Z) (n: Z) (i: Z) (retval: Z) (PreH1 : (retval = 0)) (PreH2 : (strstr_result a_l (rotate_at_154 (b_l) (i)) retval a0 )) (PreH3 : (0 <= ((string_length ((rotate_at_154 (b_l) (i)))) + 1 ))) (PreH4 : (0 <= ((string_length (b_l)) + 1 ))) (PreH5 : (0 <= ((string_length (a_l)) + 1 ))) (PreH6 : (rotate <> 0)) (PreH7 : ((n + 1 ) < INT_MAX)) (PreH8 : (valid_string a_l )) (PreH9 : (valid_string b_l )) (PreH10 : ((string_length (a_l)) < INT_MAX)) (PreH11 : (n = (string_length (b_l)))) (PreH12 : (rotation_scan_state_154 a_l b_l i )) (PreH13 : (rotation_prefix_154 b_l i n (rotate_at_154 (b_l) (i)) )) (PreH14 : (valid_string (rotate_at_154 (b_l) (i)) )) ,
+  (CharArray.full rotate ((string_length ((rotate_at_154 (b_l) (i)))) + 1 ) (c_string ((rotate_at_154 (b_l) (i)))) )
+|--
+  “ (rotation_scan_state_154 a_l b_l (i + 1 ) ) ”
+  &&  (CharArray.undef_full rotate (n + 1 ) )
+).
+
+Definition cycpattern_check_entail_wit_8_split_goal_1 := 
+forall (a0: Z) (b_l: (@list Z)) (a_l: (@list Z)) (rotate: Z) (n: Z) (i: Z) (retval: Z) (PreH1 : (retval = 0)) (PreH2 : (strstr_result a_l (rotate_at_154 (b_l) (i)) retval a0 )) (PreH3 : (0 <= ((string_length ((rotate_at_154 (b_l) (i)))) + 1 ))) (PreH4 : (0 <= ((string_length (b_l)) + 1 ))) (PreH5 : (0 <= ((string_length (a_l)) + 1 ))) (PreH6 : (rotate <> 0)) (PreH7 : ((n + 1 ) < INT_MAX)) (PreH8 : (valid_string a_l )) (PreH9 : (valid_string b_l )) (PreH10 : ((string_length (a_l)) < INT_MAX)) (PreH11 : (n = (string_length (b_l)))) (PreH12 : (rotation_scan_state_154 a_l b_l i )) (PreH13 : (rotation_prefix_154 b_l i n (rotate_at_154 (b_l) (i)) )) (PreH14 : (valid_string (rotate_at_154 (b_l) (i)) )) ,
+  (CharArray.full rotate ((string_length ((rotate_at_154 (b_l) (i)))) + 1 ) (c_string ((rotate_at_154 (b_l) (i)))) )
+|--
+  “ (rotation_scan_state_154 a_l b_l (i + 1 ) ) ”
+.
+
+Definition cycpattern_check_entail_wit_8_split_goal_spatial := 
+forall (a0: Z) (b_l: (@list Z)) (a_l: (@list Z)) (rotate: Z) (n: Z) (i: Z) (retval: Z) (PreH1 : (retval = 0)) (PreH2 : (strstr_result a_l (rotate_at_154 (b_l) (i)) retval a0 )) (PreH3 : (0 <= ((string_length ((rotate_at_154 (b_l) (i)))) + 1 ))) (PreH4 : (0 <= ((string_length (b_l)) + 1 ))) (PreH5 : (0 <= ((string_length (a_l)) + 1 ))) (PreH6 : (rotate <> 0)) (PreH7 : ((n + 1 ) < INT_MAX)) (PreH8 : (valid_string a_l )) (PreH9 : (valid_string b_l )) (PreH10 : ((string_length (a_l)) < INT_MAX)) (PreH11 : (n = (string_length (b_l)))) (PreH12 : (rotation_scan_state_154 a_l b_l i )) (PreH13 : (rotation_prefix_154 b_l i n (rotate_at_154 (b_l) (i)) )) (PreH14 : (valid_string (rotate_at_154 (b_l) (i)) )) ,
+  (CharArray.full rotate ((string_length ((rotate_at_154 (b_l) (i)))) + 1 ) (c_string ((rotate_at_154 (b_l) (i)))) )
+|--
+  (CharArray.undef_full rotate (n + 1 ) )
+.
+
+Definition cycpattern_check_entail_wit_9 := 
+(
+forall (b0: Z) (a0: Z) (b_l: (@list Z)) (a_l: (@list Z)) (hit: Z) (rotate: Z) (n: Z) (i: Z) (PreH1 : (hit = 0)) (PreH2 : (rotate <> 0)) (PreH3 : ((n + 1 ) < INT_MAX)) (PreH4 : (valid_string a_l )) (PreH5 : (valid_string b_l )) (PreH6 : ((string_length (a_l)) < INT_MAX)) (PreH7 : (n = (string_length (b_l)))) (PreH8 : (rotation_scan_state_154 a_l b_l (i + 1 ) )) ,
+  (store_string a0 a_l )
+  **  (store_string b0 b_l )
+  **  (CharArray.undef_full rotate (n + 1 ) )
+|--
+  “ (0 <= (i + 1 )) ” 
+  &&  “ ((i + 1 ) <= n) ” 
+  &&  “ (rotate <> 0) ” 
+  &&  “ ((n + 1 ) < INT_MAX) ” 
+  &&  “ (valid_string a_l ) ” 
+  &&  “ (valid_string b_l ) ” 
+  &&  “ ((string_length (a_l)) < INT_MAX) ” 
+  &&  “ (n = (string_length (b_l))) ” 
+  &&  “ (rotation_scan_state_154 a_l b_l (i + 1 ) ) ”
+  &&  (store_string a0 a_l )
+  **  (store_string b0 b_l )
+  **  (CharArray.undef_full rotate (n + 1 ) )
+) \/
+(
+forall (b_l: (@list Z)) (a_l: (@list Z)) (hit: Z) (rotate: Z) (n: Z) (i: Z) (PreH1 : (0 <= ((string_length (b_l)) + 1 ))) (PreH2 : (0 <= ((string_length (a_l)) + 1 ))) (PreH3 : (hit = 0)) (PreH4 : (rotate <> 0)) (PreH5 : ((n + 1 ) < INT_MAX)) (PreH6 : (valid_string a_l )) (PreH7 : (valid_string b_l )) (PreH8 : ((string_length (a_l)) < INT_MAX)) (PreH9 : (n = (string_length (b_l)))) (PreH10 : (rotation_scan_state_154 a_l b_l (i + 1 ) )) ,
+  (CharArray.undef_full rotate (n + 1 ) )
+|--
+  “ ((i + 1 ) <= n) ” 
+  &&  “ (0 <= (i + 1 )) ”
+  &&  (CharArray.undef_full rotate (n + 1 ) )
+).
+
+Definition cycpattern_check_entail_wit_9_split_goal_1 := 
+forall (b_l: (@list Z)) (a_l: (@list Z)) (hit: Z) (rotate: Z) (n: Z) (i: Z) (PreH1 : (0 <= ((string_length (b_l)) + 1 ))) (PreH2 : (0 <= ((string_length (a_l)) + 1 ))) (PreH3 : (hit = 0)) (PreH4 : (rotate <> 0)) (PreH5 : ((n + 1 ) < INT_MAX)) (PreH6 : (valid_string a_l )) (PreH7 : (valid_string b_l )) (PreH8 : ((string_length (a_l)) < INT_MAX)) (PreH9 : (n = (string_length (b_l)))) (PreH10 : (rotation_scan_state_154 a_l b_l (i + 1 ) )) ,
+  (CharArray.undef_full rotate (n + 1 ) )
+|--
+  “ ((i + 1 ) <= n) ”
+.
+
+Definition cycpattern_check_entail_wit_9_split_goal_2 := 
+forall (b_l: (@list Z)) (a_l: (@list Z)) (hit: Z) (rotate: Z) (n: Z) (i: Z) (PreH1 : (0 <= ((string_length (b_l)) + 1 ))) (PreH2 : (0 <= ((string_length (a_l)) + 1 ))) (PreH3 : (hit = 0)) (PreH4 : (rotate <> 0)) (PreH5 : ((n + 1 ) < INT_MAX)) (PreH6 : (valid_string a_l )) (PreH7 : (valid_string b_l )) (PreH8 : ((string_length (a_l)) < INT_MAX)) (PreH9 : (n = (string_length (b_l)))) (PreH10 : (rotation_scan_state_154 a_l b_l (i + 1 ) )) ,
+  (CharArray.undef_full rotate (n + 1 ) )
+|--
+  “ (0 <= (i + 1 )) ”
+.
+
+Definition cycpattern_check_entail_wit_9_split_goal_spatial := 
+forall (b_l: (@list Z)) (a_l: (@list Z)) (hit: Z) (rotate: Z) (n: Z) (i: Z) (PreH1 : (0 <= ((string_length (b_l)) + 1 ))) (PreH2 : (0 <= ((string_length (a_l)) + 1 ))) (PreH3 : (hit = 0)) (PreH4 : (rotate <> 0)) (PreH5 : ((n + 1 ) < INT_MAX)) (PreH6 : (valid_string a_l )) (PreH7 : (valid_string b_l )) (PreH8 : ((string_length (a_l)) < INT_MAX)) (PreH9 : (n = (string_length (b_l)))) (PreH10 : (rotation_scan_state_154 a_l b_l (i + 1 ) )) ,
+  (CharArray.undef_full rotate (n + 1 ) )
+|--
+  (CharArray.undef_full rotate (n + 1 ) )
+.
+
+Definition cycpattern_check_return_wit_1 := 
+forall (b0: Z) (a0: Z) (b_l: (@list Z)) (a_l: (@list Z)) (rotate: Z) (n: Z) (i: Z) (PreH1 : (0 <= ((string_length (b_l)) + 1 ))) (PreH2 : (0 <= ((string_length (a_l)) + 1 ))) (PreH3 : (i >= n)) (PreH4 : (0 <= i)) (PreH5 : (i <= n)) (PreH6 : (rotate <> 0)) (PreH7 : ((n + 1 ) < INT_MAX)) (PreH8 : (valid_string a_l )) (PreH9 : (valid_string b_l )) (PreH10 : ((string_length (a_l)) < INT_MAX)) (PreH11 : (n = (string_length (b_l)))) (PreH12 : (rotation_scan_state_154 a_l b_l i )) ,
+  (CharArray.full b0 ((string_length (b_l)) + 1 ) (c_string (b_l)) )
+  **  (CharArray.full a0 ((string_length (a_l)) + 1 ) (c_string (a_l)) )
+|--
+  (“ (0 = 0) ” 
+  &&  “ (problem_154_spec_z a_l b_l 0 ) ”
+  &&  (store_string a0 a_l )
+  **  (store_string b0 b_l ))
+  ||
+  (“ (0 = 1) ” 
+  &&  “ (problem_154_spec_z a_l b_l 0 ) ”
+  &&  (store_string a0 a_l )
+  **  (store_string b0 b_l ))
+.
+
+Definition cycpattern_check_return_wit_2 := 
+forall (b0: Z) (a0: Z) (b_l: (@list Z)) (a_l: (@list Z)) (hit: Z) (rotate: Z) (n: Z) (i: Z) (PreH1 : (0 <= ((string_length (b_l)) + 1 ))) (PreH2 : (0 <= ((string_length (a_l)) + 1 ))) (PreH3 : (hit <> 0)) (PreH4 : (rotate <> 0)) (PreH5 : ((n + 1 ) < INT_MAX)) (PreH6 : (valid_string a_l )) (PreH7 : (valid_string b_l )) (PreH8 : ((string_length (a_l)) < INT_MAX)) (PreH9 : (n = (string_length (b_l)))) (PreH10 : (rotation_success_154 a_l b_l i (rotate_at_154 (b_l) (i)) )) ,
+  (CharArray.full b0 ((string_length (b_l)) + 1 ) (c_string (b_l)) )
+  **  (CharArray.full a0 ((string_length (a_l)) + 1 ) (c_string (a_l)) )
+|--
+  (“ (1 = 0) ” 
+  &&  “ (problem_154_spec_z a_l b_l 1 ) ”
+  &&  (store_string a0 a_l )
+  **  (store_string b0 b_l ))
+  ||
+  (“ (1 = 1) ” 
+  &&  “ (problem_154_spec_z a_l b_l 1 ) ”
+  &&  (store_string a0 a_l )
+  **  (store_string b0 b_l ))
+.
+
+Definition cycpattern_check_partial_solve_wit_1_pure := 
+forall (b_pre: Z) (a_pre: Z) (b0: Z) (a0: Z) (b_l: (@list Z)) (a_l: (@list Z)) (PreH1 : (a_pre = a0)) (PreH2 : (b_pre = b0)) (PreH3 : (problem_154_pre_z a_l b_l )) (PreH4 : (valid_string a_l )) (PreH5 : (valid_string b_l )) (PreH6 : ((string_length (a_l)) < INT_MAX)) (PreH7 : (((string_length (b_l)) + 1 ) < INT_MAX)) ,
+  ((( &( "n" ) )) # Int  |->_)
+  **  ((( &( "b" ) )) # Ptr  |-> b_pre)
+  **  ((( &( "a" ) )) # Ptr  |-> a_pre)
+  **  (store_string a0 a_l )
+  **  (store_string b0 b_l )
+|--
+  “ (valid_string b_l ) ” 
+  &&  “ ((string_length (b_l)) < INT_MAX) ”
+.
+
+Definition cycpattern_check_partial_solve_wit_1_aux := 
+forall (b_pre: Z) (a_pre: Z) (b0: Z) (a0: Z) (b_l: (@list Z)) (a_l: (@list Z)) (PreH1 : (a_pre = a0)) (PreH2 : (b_pre = b0)) (PreH3 : (problem_154_pre_z a_l b_l )) (PreH4 : (valid_string a_l )) (PreH5 : (valid_string b_l )) (PreH6 : ((string_length (a_l)) < INT_MAX)) (PreH7 : (((string_length (b_l)) + 1 ) < INT_MAX)) ,
+  (store_string a0 a_l )
+  **  (store_string b0 b_l )
+|--
+  “ (valid_string b_l ) ” 
+  &&  “ ((string_length (b_l)) < INT_MAX) ” 
+  &&  “ (0 <= ((string_length (b_l)) + 1 )) ” 
+  &&  “ (0 <= ((string_length (a_l)) + 1 )) ” 
+  &&  “ (a_pre = a0) ” 
+  &&  “ (b_pre = b0) ” 
+  &&  “ (problem_154_pre_z a_l b_l ) ” 
+  &&  “ (valid_string a_l ) ” 
+  &&  “ (valid_string b_l ) ” 
+  &&  “ ((string_length (a_l)) < INT_MAX) ” 
+  &&  “ (((string_length (b_l)) + 1 ) < INT_MAX) ”
+  &&  (store_string b_pre b_l )
+  **  (CharArray.full a0 ((string_length (a_l)) + 1 ) (c_string (a_l)) )
+.
+
+Definition cycpattern_check_partial_solve_wit_1 := cycpattern_check_partial_solve_wit_1_pure -> cycpattern_check_partial_solve_wit_1_aux.
+
+Definition cycpattern_check_partial_solve_wit_2_pure := 
+forall (b_pre: Z) (a_pre: Z) (b0: Z) (a0: Z) (b_l: (@list Z)) (a_l: (@list Z)) (retval: Z) (PreH1 : (retval = (string_length (b_l)))) (PreH2 : (0 <= ((string_length (b_l)) + 1 ))) (PreH3 : (0 <= ((string_length (a_l)) + 1 ))) (PreH4 : (a_pre = a0)) (PreH5 : (b_pre = b0)) (PreH6 : (problem_154_pre_z a_l b_l )) (PreH7 : (valid_string a_l )) (PreH8 : (valid_string b_l )) (PreH9 : ((string_length (a_l)) < INT_MAX)) (PreH10 : (((string_length (b_l)) + 1 ) < INT_MAX)) ,
+  ((( &( "rotate" ) )) # Ptr  |->_)
+  **  (store_string b_pre b_l )
+  **  (CharArray.full a0 ((string_length (a_l)) + 1 ) (c_string (a_l)) )
+  **  ((( &( "n" ) )) # Int  |-> retval)
+  **  ((( &( "b" ) )) # Ptr  |-> b_pre)
+  **  ((( &( "a" ) )) # Ptr  |-> a_pre)
+|--
+  “ (0 <= (retval + 1 )) ” 
+  &&  “ ((retval + 1 ) < INT_MAX) ”
+.
+
+Definition cycpattern_check_partial_solve_wit_2_aux := 
+forall (b_pre: Z) (a_pre: Z) (b0: Z) (a0: Z) (b_l: (@list Z)) (a_l: (@list Z)) (retval: Z) (PreH1 : (retval = (string_length (b_l)))) (PreH2 : (0 <= ((string_length (b_l)) + 1 ))) (PreH3 : (0 <= ((string_length (a_l)) + 1 ))) (PreH4 : (a_pre = a0)) (PreH5 : (b_pre = b0)) (PreH6 : (problem_154_pre_z a_l b_l )) (PreH7 : (valid_string a_l )) (PreH8 : (valid_string b_l )) (PreH9 : ((string_length (a_l)) < INT_MAX)) (PreH10 : (((string_length (b_l)) + 1 ) < INT_MAX)) ,
+  (store_string b_pre b_l )
+  **  (CharArray.full a0 ((string_length (a_l)) + 1 ) (c_string (a_l)) )
+|--
+  “ (0 <= (retval + 1 )) ” 
+  &&  “ ((retval + 1 ) < INT_MAX) ” 
+  &&  “ (retval = (string_length (b_l))) ” 
+  &&  “ (0 <= ((string_length (b_l)) + 1 )) ” 
+  &&  “ (0 <= ((string_length (a_l)) + 1 )) ” 
+  &&  “ (a_pre = a0) ” 
+  &&  “ (b_pre = b0) ” 
+  &&  “ (problem_154_pre_z a_l b_l ) ” 
+  &&  “ (valid_string a_l ) ” 
+  &&  “ (valid_string b_l ) ” 
+  &&  “ ((string_length (a_l)) < INT_MAX) ” 
+  &&  “ (((string_length (b_l)) + 1 ) < INT_MAX) ”
+  &&  (CharArray.full b_pre ((string_length (b_l)) + 1 ) (c_string (b_l)) )
+  **  (CharArray.full a0 ((string_length (a_l)) + 1 ) (c_string (a_l)) )
+.
+
+Definition cycpattern_check_partial_solve_wit_2 := cycpattern_check_partial_solve_wit_2_pure -> cycpattern_check_partial_solve_wit_2_aux.
+
+Definition cycpattern_check_partial_solve_wit_3 := 
+forall (b0: Z) (a0: Z) (b_l: (@list Z)) (a_l: (@list Z)) (rotate_l: (@list Z)) (ch: Z) (idx: Z) (i: Z) (j: Z) (n: Z) (rotate: Z) (PreH1 : (ch = (Znth (idx) (b_l) (0)))) (PreH2 : (idx = ((i + j ) % ( n ) ))) (PreH3 : (0 <= ch)) (PreH4 : (ch <= 127)) (PreH5 : (0 <= idx)) (PreH6 : (idx < n)) (PreH7 : (0 <= j)) (PreH8 : (j < n)) (PreH9 : (0 < n)) (PreH10 : (0 <= i)) (PreH11 : (i < n)) (PreH12 : (rotate <> 0)) (PreH13 : ((n + 1 ) < INT_MAX)) (PreH14 : (valid_string a_l )) (PreH15 : (valid_string b_l )) (PreH16 : ((string_length (a_l)) < INT_MAX)) (PreH17 : (n = (string_length (b_l)))) (PreH18 : (rotation_scan_state_154 a_l b_l i )) (PreH19 : (rotation_prefix_154 b_l i j rotate_l )) ,
+  (store_string a0 a_l )
+  **  (store_string b0 b_l )
+  **  (CharArray.full rotate j rotate_l )
+  **  (CharArray.undef_seg rotate j (n + 1 ) )
+|--
+  “ (0 <= ((string_length (b_l)) + 1 )) ” 
+  &&  “ (0 <= ((string_length (a_l)) + 1 )) ” 
+  &&  “ (ch = (Znth (idx) (b_l) (0))) ” 
+  &&  “ (idx = ((i + j ) % ( n ) )) ” 
+  &&  “ (0 <= ch) ” 
+  &&  “ (ch <= 127) ” 
+  &&  “ (0 <= idx) ” 
+  &&  “ (idx < n) ” 
+  &&  “ (0 <= j) ” 
+  &&  “ (j < n) ” 
+  &&  “ (0 < n) ” 
+  &&  “ (0 <= i) ” 
+  &&  “ (i < n) ” 
+  &&  “ (rotate <> 0) ” 
+  &&  “ ((n + 1 ) < INT_MAX) ” 
+  &&  “ (valid_string a_l ) ” 
+  &&  “ (valid_string b_l ) ” 
+  &&  “ ((string_length (a_l)) < INT_MAX) ” 
+  &&  “ (n = (string_length (b_l))) ” 
+  &&  “ (rotation_scan_state_154 a_l b_l i ) ” 
+  &&  “ (rotation_prefix_154 b_l i j rotate_l ) ”
+  &&  (((rotate + (j * sizeof(CHAR) ) )) # Char  |->_)
+  **  (CharArray.full b0 ((string_length (b_l)) + 1 ) (c_string (b_l)) )
+  **  (CharArray.full a0 ((string_length (a_l)) + 1 ) (c_string (a_l)) )
+  **  (CharArray.undef_missing_i rotate j j (n + 1 ) )
+  **  (CharArray.full rotate j rotate_l )
+.
+
+Definition cycpattern_check_partial_solve_wit_4 := 
+forall (b0: Z) (a0: Z) (b_l: (@list Z)) (a_l: (@list Z)) (rotate_l: (@list Z)) (rotate: Z) (i: Z) (n: Z) (j: Z) (PreH1 : (j >= n)) (PreH2 : (0 <= j)) (PreH3 : (j <= n)) (PreH4 : (0 < n)) (PreH5 : (0 <= i)) (PreH6 : (i < n)) (PreH7 : (rotate <> 0)) (PreH8 : ((n + 1 ) < INT_MAX)) (PreH9 : (valid_string a_l )) (PreH10 : (valid_string b_l )) (PreH11 : ((string_length (a_l)) < INT_MAX)) (PreH12 : (n = (string_length (b_l)))) (PreH13 : (rotation_scan_state_154 a_l b_l i )) (PreH14 : (rotation_prefix_154 b_l i j rotate_l )) ,
+  (store_string a0 a_l )
+  **  (store_string b0 b_l )
+  **  (CharArray.full rotate j rotate_l )
+  **  (CharArray.undef_seg rotate j (n + 1 ) )
+|--
+  “ (0 <= ((string_length (b_l)) + 1 )) ” 
+  &&  “ (0 <= ((string_length (a_l)) + 1 )) ” 
+  &&  “ (j >= n) ” 
+  &&  “ (0 <= j) ” 
+  &&  “ (j <= n) ” 
+  &&  “ (0 < n) ” 
+  &&  “ (0 <= i) ” 
+  &&  “ (i < n) ” 
+  &&  “ (rotate <> 0) ” 
+  &&  “ ((n + 1 ) < INT_MAX) ” 
+  &&  “ (valid_string a_l ) ” 
+  &&  “ (valid_string b_l ) ” 
+  &&  “ ((string_length (a_l)) < INT_MAX) ” 
+  &&  “ (n = (string_length (b_l))) ” 
+  &&  “ (rotation_scan_state_154 a_l b_l i ) ” 
+  &&  “ (rotation_prefix_154 b_l i j rotate_l ) ”
+  &&  (((rotate + (n * sizeof(CHAR) ) )) # Char  |->_)
+  **  (CharArray.full b0 ((string_length (b_l)) + 1 ) (c_string (b_l)) )
+  **  (CharArray.full a0 ((string_length (a_l)) + 1 ) (c_string (a_l)) )
+  **  (CharArray.undef_missing_i rotate n j (n + 1 ) )
+  **  (CharArray.full rotate j rotate_l )
+.
+
+Definition cycpattern_check_partial_solve_wit_5_pure := 
+(
+forall (b0: Z) (a0: Z) (b_l: (@list Z)) (a_l: (@list Z)) (rotate: Z) (n: Z) (i: Z) (PreH1 : (rotate <> 0)) (PreH2 : ((n + 1 ) < INT_MAX)) (PreH3 : (valid_string a_l )) (PreH4 : (valid_string b_l )) (PreH5 : ((string_length (a_l)) < INT_MAX)) (PreH6 : (n = (string_length (b_l)))) (PreH7 : (rotation_scan_state_154 a_l b_l i )) (PreH8 : (rotation_prefix_154 b_l i n (rotate_at_154 (b_l) (i)) )) (PreH9 : (valid_string (rotate_at_154 (b_l) (i)) )) ,
+  ((( &( "hit" ) )) # Ptr  |->_)
+  **  ((( &( "rotate" ) )) # Ptr  |-> rotate)
+  **  ((( &( "n" ) )) # Int  |-> n)
+  **  ((( &( "a" ) )) # Ptr  |-> a0)
+  **  ((( &( "b" ) )) # Ptr  |-> b0)
+  **  ((( &( "i" ) )) # Int  |-> i)
+  **  (store_string a0 a_l )
+  **  (store_string b0 b_l )
+  **  (store_string rotate (rotate_at_154 (b_l) (i)) )
+|--
+  “ (valid_string a_l ) ” 
+  &&  “ (valid_string (rotate_at_154 (b_l) (i)) ) ” 
+  &&  “ ((string_length (a_l)) < INT_MAX) ” 
+  &&  “ ((string_length ((rotate_at_154 (b_l) (i)))) < INT_MAX) ”
+) \/
+(
+forall (b0: Z) (a0: Z) (b_l: (@list Z)) (a_l: (@list Z)) (rotate: Z) (n: Z) (i: Z) (PreH1 : (i <= INT_MAX)) (PreH2 : (n <= INT_MAX)) (PreH3 : (i >= INT_MIN)) (PreH4 : (n >= INT_MIN)) (PreH5 : (0 <= ((string_length ((rotate_at_154 (b_l) (i)))) + 1 ))) (PreH6 : (0 <= ((string_length (b_l)) + 1 ))) (PreH7 : (0 <= ((string_length (a_l)) + 1 ))) (PreH8 : (rotate <> 0)) (PreH9 : ((n + 1 ) < INT_MAX)) (PreH10 : (valid_string a_l )) (PreH11 : (valid_string b_l )) (PreH12 : ((string_length (a_l)) < INT_MAX)) (PreH13 : (n = (string_length (b_l)))) (PreH14 : (rotation_scan_state_154 a_l b_l i )) (PreH15 : (rotation_prefix_154 b_l i n (rotate_at_154 (b_l) (i)) )) (PreH16 : (valid_string (rotate_at_154 (b_l) (i)) )) ,
+  (CharArray.full rotate ((string_length ((rotate_at_154 (b_l) (i)))) + 1 ) (c_string ((rotate_at_154 (b_l) (i)))) )
+  **  (CharArray.full b0 ((string_length (b_l)) + 1 ) (c_string (b_l)) )
+  **  (CharArray.full a0 ((string_length (a_l)) + 1 ) (c_string (a_l)) )
+  **  ((( &( "hit" ) )) # Ptr  |->_)
+  **  ((( &( "rotate" ) )) # Ptr  |-> rotate)
+  **  ((( &( "n" ) )) # Int  |-> n)
+  **  ((( &( "a" ) )) # Ptr  |-> a0)
+  **  ((( &( "b" ) )) # Ptr  |-> b0)
+  **  ((( &( "i" ) )) # Int  |-> i)
+|--
+  “ ((string_length ((rotate_at_154 (b_l) (i)))) < INT_MAX) ”
+).
+
+Definition cycpattern_check_partial_solve_wit_5_pure_split_goal_1 := 
+forall (b0: Z) (a0: Z) (b_l: (@list Z)) (a_l: (@list Z)) (rotate: Z) (n: Z) (i: Z) (PreH1 : (i <= INT_MAX)) (PreH2 : (n <= INT_MAX)) (PreH3 : (i >= INT_MIN)) (PreH4 : (n >= INT_MIN)) (PreH5 : (0 <= ((string_length ((rotate_at_154 (b_l) (i)))) + 1 ))) (PreH6 : (0 <= ((string_length (b_l)) + 1 ))) (PreH7 : (0 <= ((string_length (a_l)) + 1 ))) (PreH8 : (rotate <> 0)) (PreH9 : ((n + 1 ) < INT_MAX)) (PreH10 : (valid_string a_l )) (PreH11 : (valid_string b_l )) (PreH12 : ((string_length (a_l)) < INT_MAX)) (PreH13 : (n = (string_length (b_l)))) (PreH14 : (rotation_scan_state_154 a_l b_l i )) (PreH15 : (rotation_prefix_154 b_l i n (rotate_at_154 (b_l) (i)) )) (PreH16 : (valid_string (rotate_at_154 (b_l) (i)) )) ,
+  (CharArray.full rotate ((string_length ((rotate_at_154 (b_l) (i)))) + 1 ) (c_string ((rotate_at_154 (b_l) (i)))) )
+  **  (CharArray.full b0 ((string_length (b_l)) + 1 ) (c_string (b_l)) )
+  **  (CharArray.full a0 ((string_length (a_l)) + 1 ) (c_string (a_l)) )
+  **  ((( &( "hit" ) )) # Ptr  |->_)
+  **  ((( &( "rotate" ) )) # Ptr  |-> rotate)
+  **  ((( &( "n" ) )) # Int  |-> n)
+  **  ((( &( "a" ) )) # Ptr  |-> a0)
+  **  ((( &( "b" ) )) # Ptr  |-> b0)
+  **  ((( &( "i" ) )) # Int  |-> i)
+|--
+  “ ((string_length ((rotate_at_154 (b_l) (i)))) < INT_MAX) ”
+.
+
+Definition cycpattern_check_partial_solve_wit_5_aux := 
+forall (b0: Z) (a0: Z) (b_l: (@list Z)) (a_l: (@list Z)) (rotate: Z) (n: Z) (i: Z) (PreH1 : (rotate <> 0)) (PreH2 : ((n + 1 ) < INT_MAX)) (PreH3 : (valid_string a_l )) (PreH4 : (valid_string b_l )) (PreH5 : ((string_length (a_l)) < INT_MAX)) (PreH6 : (n = (string_length (b_l)))) (PreH7 : (rotation_scan_state_154 a_l b_l i )) (PreH8 : (rotation_prefix_154 b_l i n (rotate_at_154 (b_l) (i)) )) (PreH9 : (valid_string (rotate_at_154 (b_l) (i)) )) ,
+  (store_string a0 a_l )
+  **  (store_string b0 b_l )
+  **  (store_string rotate (rotate_at_154 (b_l) (i)) )
+|--
+  “ (valid_string a_l ) ” 
+  &&  “ (valid_string (rotate_at_154 (b_l) (i)) ) ” 
+  &&  “ ((string_length (a_l)) < INT_MAX) ” 
+  &&  “ ((string_length ((rotate_at_154 (b_l) (i)))) < INT_MAX) ” 
+  &&  “ (0 <= ((string_length ((rotate_at_154 (b_l) (i)))) + 1 )) ” 
+  &&  “ (0 <= ((string_length (b_l)) + 1 )) ” 
+  &&  “ (0 <= ((string_length (a_l)) + 1 )) ” 
+  &&  “ (rotate <> 0) ” 
+  &&  “ ((n + 1 ) < INT_MAX) ” 
+  &&  “ (valid_string a_l ) ” 
+  &&  “ (valid_string b_l ) ” 
+  &&  “ ((string_length (a_l)) < INT_MAX) ” 
+  &&  “ (n = (string_length (b_l))) ” 
+  &&  “ (rotation_scan_state_154 a_l b_l i ) ” 
+  &&  “ (rotation_prefix_154 b_l i n (rotate_at_154 (b_l) (i)) ) ” 
+  &&  “ (valid_string (rotate_at_154 (b_l) (i)) ) ”
+  &&  (store_string a0 a_l )
+  **  (store_string rotate (rotate_at_154 (b_l) (i)) )
+  **  (CharArray.full b0 ((string_length (b_l)) + 1 ) (c_string (b_l)) )
+.
+
+Definition cycpattern_check_partial_solve_wit_5 := cycpattern_check_partial_solve_wit_5_pure -> cycpattern_check_partial_solve_wit_5_aux.
+
+Definition cycpattern_check_partial_solve_wit_6_pure := 
+forall (b0: Z) (a0: Z) (b_l: (@list Z)) (a_l: (@list Z)) (hit: Z) (rotate: Z) (n: Z) (i: Z) (PreH1 : (hit <> 0)) (PreH2 : (rotate <> 0)) (PreH3 : ((n + 1 ) < INT_MAX)) (PreH4 : (valid_string a_l )) (PreH5 : (valid_string b_l )) (PreH6 : ((string_length (a_l)) < INT_MAX)) (PreH7 : (n = (string_length (b_l)))) (PreH8 : (rotation_success_154 a_l b_l i (rotate_at_154 (b_l) (i)) )) ,
+  ((( &( "hit" ) )) # Ptr  |-> hit)
+  **  ((( &( "rotate" ) )) # Ptr  |-> rotate)
+  **  ((( &( "n" ) )) # Int  |-> n)
+  **  ((( &( "a" ) )) # Ptr  |-> a0)
+  **  ((( &( "b" ) )) # Ptr  |-> b0)
+  **  ((( &( "i" ) )) # Int  |-> i)
+  **  (store_string a0 a_l )
+  **  (store_string b0 b_l )
+  **  (CharArray.undef_full rotate (n + 1 ) )
+|--
+  “ (rotate <> 0) ” 
+  &&  “ (0 <= (n + 1 )) ” 
+  &&  “ ((n + 1 ) < INT_MAX) ”
+.
+
+Definition cycpattern_check_partial_solve_wit_6_aux := 
+forall (b0: Z) (a0: Z) (b_l: (@list Z)) (a_l: (@list Z)) (hit: Z) (rotate: Z) (n: Z) (i: Z) (PreH1 : (hit <> 0)) (PreH2 : (rotate <> 0)) (PreH3 : ((n + 1 ) < INT_MAX)) (PreH4 : (valid_string a_l )) (PreH5 : (valid_string b_l )) (PreH6 : ((string_length (a_l)) < INT_MAX)) (PreH7 : (n = (string_length (b_l)))) (PreH8 : (rotation_success_154 a_l b_l i (rotate_at_154 (b_l) (i)) )) ,
+  (store_string a0 a_l )
+  **  (store_string b0 b_l )
+  **  (CharArray.undef_full rotate (n + 1 ) )
+|--
+  “ (rotate <> 0) ” 
+  &&  “ (0 <= (n + 1 )) ” 
+  &&  “ ((n + 1 ) < INT_MAX) ” 
+  &&  “ (0 <= ((string_length (b_l)) + 1 )) ” 
+  &&  “ (0 <= ((string_length (a_l)) + 1 )) ” 
+  &&  “ (hit <> 0) ” 
+  &&  “ (rotate <> 0) ” 
+  &&  “ ((n + 1 ) < INT_MAX) ” 
+  &&  “ (valid_string a_l ) ” 
+  &&  “ (valid_string b_l ) ” 
+  &&  “ ((string_length (a_l)) < INT_MAX) ” 
+  &&  “ (n = (string_length (b_l))) ” 
+  &&  “ (rotation_success_154 a_l b_l i (rotate_at_154 (b_l) (i)) ) ”
+  &&  (CharArray.undef_full rotate (n + 1 ) )
+  **  (CharArray.full b0 ((string_length (b_l)) + 1 ) (c_string (b_l)) )
+  **  (CharArray.full a0 ((string_length (a_l)) + 1 ) (c_string (a_l)) )
+.
+
+Definition cycpattern_check_partial_solve_wit_6 := cycpattern_check_partial_solve_wit_6_pure -> cycpattern_check_partial_solve_wit_6_aux.
+
+Definition cycpattern_check_partial_solve_wit_7_pure := 
+forall (b0: Z) (a0: Z) (b_l: (@list Z)) (a_l: (@list Z)) (rotate: Z) (n: Z) (i: Z) (PreH1 : (i >= n)) (PreH2 : (0 <= i)) (PreH3 : (i <= n)) (PreH4 : (rotate <> 0)) (PreH5 : ((n + 1 ) < INT_MAX)) (PreH6 : (valid_string a_l )) (PreH7 : (valid_string b_l )) (PreH8 : ((string_length (a_l)) < INT_MAX)) (PreH9 : (n = (string_length (b_l)))) (PreH10 : (rotation_scan_state_154 a_l b_l i )) ,
+  ((( &( "i" ) )) # Int  |-> i)
+  **  ((( &( "n" ) )) # Int  |-> n)
+  **  ((( &( "rotate" ) )) # Ptr  |-> rotate)
+  **  ((( &( "a" ) )) # Ptr  |-> a0)
+  **  ((( &( "b" ) )) # Ptr  |-> b0)
+  **  (store_string a0 a_l )
+  **  (store_string b0 b_l )
+  **  (CharArray.undef_full rotate (n + 1 ) )
+|--
+  “ (rotate <> 0) ” 
+  &&  “ (0 <= (n + 1 )) ” 
+  &&  “ ((n + 1 ) < INT_MAX) ”
+.
+
+Definition cycpattern_check_partial_solve_wit_7_aux := 
+forall (b0: Z) (a0: Z) (b_l: (@list Z)) (a_l: (@list Z)) (rotate: Z) (n: Z) (i: Z) (PreH1 : (i >= n)) (PreH2 : (0 <= i)) (PreH3 : (i <= n)) (PreH4 : (rotate <> 0)) (PreH5 : ((n + 1 ) < INT_MAX)) (PreH6 : (valid_string a_l )) (PreH7 : (valid_string b_l )) (PreH8 : ((string_length (a_l)) < INT_MAX)) (PreH9 : (n = (string_length (b_l)))) (PreH10 : (rotation_scan_state_154 a_l b_l i )) ,
+  (store_string a0 a_l )
+  **  (store_string b0 b_l )
+  **  (CharArray.undef_full rotate (n + 1 ) )
+|--
+  “ (rotate <> 0) ” 
+  &&  “ (0 <= (n + 1 )) ” 
+  &&  “ ((n + 1 ) < INT_MAX) ” 
+  &&  “ (0 <= ((string_length (b_l)) + 1 )) ” 
+  &&  “ (0 <= ((string_length (a_l)) + 1 )) ” 
+  &&  “ (i >= n) ” 
+  &&  “ (0 <= i) ” 
+  &&  “ (i <= n) ” 
+  &&  “ (rotate <> 0) ” 
+  &&  “ ((n + 1 ) < INT_MAX) ” 
+  &&  “ (valid_string a_l ) ” 
+  &&  “ (valid_string b_l ) ” 
+  &&  “ ((string_length (a_l)) < INT_MAX) ” 
+  &&  “ (n = (string_length (b_l))) ” 
+  &&  “ (rotation_scan_state_154 a_l b_l i ) ”
+  &&  (CharArray.undef_full rotate (n + 1 ) )
+  **  (CharArray.full b0 ((string_length (b_l)) + 1 ) (c_string (b_l)) )
+  **  (CharArray.full a0 ((string_length (a_l)) + 1 ) (c_string (a_l)) )
+.
+
+Definition cycpattern_check_partial_solve_wit_7 := cycpattern_check_partial_solve_wit_7_pure -> cycpattern_check_partial_solve_wit_7_aux.
+
+Module Type VC_Correct.
+
+Include char_array_Strategy_Correct.
+Include string_Strategy_Correct.
+
+Axiom proof_of_cycpattern_check_safety_wit_1 : cycpattern_check_safety_wit_1.
+Axiom proof_of_cycpattern_check_safety_wit_2 : cycpattern_check_safety_wit_2.
+Axiom proof_of_cycpattern_check_safety_wit_3 : cycpattern_check_safety_wit_3.
+Axiom proof_of_cycpattern_check_safety_wit_4 : cycpattern_check_safety_wit_4.
+Axiom proof_of_cycpattern_check_safety_wit_5 : cycpattern_check_safety_wit_5.
+Axiom proof_of_cycpattern_check_safety_wit_6 : cycpattern_check_safety_wit_6.
+Axiom proof_of_cycpattern_check_safety_wit_7 : cycpattern_check_safety_wit_7.
+Axiom proof_of_cycpattern_check_safety_wit_8 : cycpattern_check_safety_wit_8.
+Axiom proof_of_cycpattern_check_safety_wit_9 : cycpattern_check_safety_wit_9.
+Axiom proof_of_cycpattern_check_safety_wit_10 : cycpattern_check_safety_wit_10.
+Axiom proof_of_cycpattern_check_safety_wit_11 : cycpattern_check_safety_wit_11.
+Axiom proof_of_cycpattern_check_safety_wit_12 : cycpattern_check_safety_wit_12.
+Axiom proof_of_cycpattern_check_safety_wit_13 : cycpattern_check_safety_wit_13.
+Axiom proof_of_cycpattern_check_safety_wit_14 : cycpattern_check_safety_wit_14.
+Axiom proof_of_cycpattern_check_safety_wit_15 : cycpattern_check_safety_wit_15.
+Axiom proof_of_cycpattern_check_safety_wit_16 : cycpattern_check_safety_wit_16.
+Axiom proof_of_cycpattern_check_safety_wit_17 : cycpattern_check_safety_wit_17.
+Axiom proof_of_cycpattern_check_safety_wit_18 : cycpattern_check_safety_wit_18.
+Axiom proof_of_cycpattern_check_safety_wit_19 : cycpattern_check_safety_wit_19.
+Axiom proof_of_cycpattern_check_safety_wit_20 : cycpattern_check_safety_wit_20.
+Axiom proof_of_cycpattern_check_entail_wit_1 : cycpattern_check_entail_wit_1.
+Axiom proof_of_cycpattern_check_entail_wit_2 : cycpattern_check_entail_wit_2.
+Axiom proof_of_cycpattern_check_entail_wit_3_1 : cycpattern_check_entail_wit_3_1.
+Axiom proof_of_cycpattern_check_entail_wit_3_2 : cycpattern_check_entail_wit_3_2.
+Axiom proof_of_cycpattern_check_entail_wit_4 : cycpattern_check_entail_wit_4.
+Axiom proof_of_cycpattern_check_entail_wit_5 : cycpattern_check_entail_wit_5.
+Axiom proof_of_cycpattern_check_entail_wit_6 : cycpattern_check_entail_wit_6.
+Axiom proof_of_cycpattern_check_entail_wit_7 : cycpattern_check_entail_wit_7.
+Axiom proof_of_cycpattern_check_entail_wit_8 : cycpattern_check_entail_wit_8.
+Axiom proof_of_cycpattern_check_entail_wit_9 : cycpattern_check_entail_wit_9.
+Axiom proof_of_cycpattern_check_return_wit_1 : cycpattern_check_return_wit_1.
+Axiom proof_of_cycpattern_check_return_wit_2 : cycpattern_check_return_wit_2.
+Axiom proof_of_cycpattern_check_partial_solve_wit_1_pure : cycpattern_check_partial_solve_wit_1_pure.
+Axiom proof_of_cycpattern_check_partial_solve_wit_1 : cycpattern_check_partial_solve_wit_1.
+Axiom proof_of_cycpattern_check_partial_solve_wit_2_pure : cycpattern_check_partial_solve_wit_2_pure.
+Axiom proof_of_cycpattern_check_partial_solve_wit_2 : cycpattern_check_partial_solve_wit_2.
+Axiom proof_of_cycpattern_check_partial_solve_wit_3 : cycpattern_check_partial_solve_wit_3.
+Axiom proof_of_cycpattern_check_partial_solve_wit_4 : cycpattern_check_partial_solve_wit_4.
+Axiom proof_of_cycpattern_check_partial_solve_wit_5_pure : cycpattern_check_partial_solve_wit_5_pure.
+Axiom proof_of_cycpattern_check_partial_solve_wit_5 : cycpattern_check_partial_solve_wit_5.
+Axiom proof_of_cycpattern_check_partial_solve_wit_6_pure : cycpattern_check_partial_solve_wit_6_pure.
+Axiom proof_of_cycpattern_check_partial_solve_wit_6 : cycpattern_check_partial_solve_wit_6.
+Axiom proof_of_cycpattern_check_partial_solve_wit_7_pure : cycpattern_check_partial_solve_wit_7_pure.
+Axiom proof_of_cycpattern_check_partial_solve_wit_7 : cycpattern_check_partial_solve_wit_7.
+
+End VC_Correct.
