QCP_examples/humaneval/spec_logic_rewrite_c_files/C_154_proof_manual.v
@@ -1,0 +1,180 @@
+Require Import Coq.ZArith.ZArith.
+Require Import Coq.Bool.Bool.
+Require Import Coq.Strings.String.
+Require Import Coq.Strings.Ascii.
+Require Import Coq.Lists.List.
+Require Import Coq.Classes.RelationClasses.
+Require Import Coq.Classes.Morphisms.
+Require Import Coq.micromega.Psatz.
+Require Import Coq.Sorting.Permutation.
+From AUXLib Require Import int_auto Axioms Feq Idents ListLib VMap.
+Require Import SetsClass.SetsClass. Import SetsNotation.
+From SimpleC.SL Require Import Mem SeparationLogic.
+From SimpleC.EE Require Import C_154_goal.
+From SimpleC.EE Require Import C_154_proof_auto.
+Require Import Logic.LogicGenerator.demo932.Interface.
+Local Open Scope Z_scope.
+Local Open Scope sets.
+Local Open Scope string_scope.
+Local Open Scope list.
+Import naive_C_Rules.
+Require Import SimpleC.StdLib.string_lib.
+Require Import coins_154.
+Local Open Scope sac.
+
+Lemma proof_of_cycpattern_check_safety_wit_17 : cycpattern_check_safety_wit_17.
+Proof.
+  right; pre_process; entailer!.
+  all: unfold rotation_scan_state_154 in PreH8;
+       destruct PreH8 as [[Hlo Hhi] Hrest];
+       unfold string_length in *;
+       pose proof (Zlength_nonneg b_l); lia.
+Qed.
+
+Lemma proof_of_cycpattern_check_entail_wit_1 : cycpattern_check_entail_wit_1.
+Proof.
+  right; pre_process; subst a_pre b_pre; entailer!.
+  - subst retval; pose proof (Zlength_nonneg b_l);
+      unfold string_length in *; entailer!.
+  - pose proof (rotation_scan_state_154_zero a_l b_l); entailer!.
+Qed.
+
+Lemma proof_of_cycpattern_check_entail_wit_2 : cycpattern_check_entail_wit_2.
+Proof.
+  right; pre_process; entailer!.
+  apply rotation_prefix_154_zero.
+  unfold string_length in PreH11; lia.
+Qed.
+
+Lemma proof_of_cycpattern_check_entail_wit_3_1 : cycpattern_check_entail_wit_3_1.
+Proof.
+  right; pre_process; entailer!.
+  rewrite Z.rem_small by lia; reflexivity.
+Qed.
+
+Lemma proof_of_cycpattern_check_entail_wit_3_2 : cycpattern_check_entail_wit_3_2.
+Proof.
+  right; pre_process; entailer!.
+  replace (i + j) with ((j - (n - i)) + 1 * n) by lia.
+  rewrite Z.rem_add by nia.
+  rewrite Z.rem_small by lia.
+  lia.
+Qed.
+
+Lemma proof_of_cycpattern_check_entail_wit_4 : cycpattern_check_entail_wit_4.
+Proof.
+  right; pre_process; entailer!.
+  all: rewrite c_string_Znth_inside by
+      (unfold string_length in *; lia).
+  - reflexivity.
+  - destruct PreH14 as [Hall Hnul]; apply Hall;
+      unfold string_length in *; lia.
+  - destruct PreH14 as [Hall Hnul]; apply Hall;
+      unfold string_length in *; lia.
+Qed.
+
+Lemma proof_of_cycpattern_check_entail_wit_5 : cycpattern_check_entail_wit_5.
+Proof.
+  right; pre_process.
+  assert (Hremmod : Z.rem (i + j) n = (i + j) mod n).
+  { apply Z.rem_mod_nonneg; lia. }
+  entailer!.
+  eapply rotation_prefix_154_step; [exact PreH21 | |].
+  - unfold string_length in PreH19; lia.
+  - unfold string_length in PreH19.
+    rewrite <- PreH19, <- Hremmod, <- PreH4; exact PreH3.
+Qed.
+
+Lemma proof_of_cycpattern_check_entail_wit_6 : cycpattern_check_entail_wit_6.
+Proof.
+  right; pre_process; entailer!.
+  all: assert (Hjn : j = n) by lia; subst j;
+       unfold rotation_prefix_154 in PreH17;
+       destruct PreH17 as [Hi [Hj Hout]];
+       assert (Hlen : Zlength (rotate_at_154 b_l i) = Zlength b_l)
+         by (apply rotate_at_154_length; lia);
+       unfold string_length in PreH15;
+       rewrite sublist_self in Hout by lia;
+       subst rotate_l.
+  - unfold store_string, string_length, c_string in *.
+    rewrite Hlen; rewrite <- PreH15; entailer!.
+  - unfold rotation_prefix_154; repeat split; try lia.
+    rewrite sublist_self by lia; reflexivity.
+  - apply valid_string_rotate_at_154; [exact PreH13 | lia].
+Qed.
+
+Lemma proof_of_cycpattern_check_entail_wit_7 : cycpattern_check_entail_wit_7.
+Proof.
+  right; pre_process; entailer!.
+  - unfold string_length in *.
+    assert (Hi : 0 <= i <= Zlength b_l).
+    { unfold rotation_prefix_154 in PreH13;
+      destruct PreH13 as [Hi0 Hrest]; lia. }
+    rewrite rotate_at_154_length by exact Hi.
+    rewrite <- PreH11.
+    apply CharArray.full_to_undef_full.
+  - split.
+    + unfold string_length in PreH11; rewrite <- PreH11; exact PreH13.
+    + exact (strstr_result_154_success a_l (rotate_at_154 b_l i)
+               retval a0 PreH1 PreH2).
+Qed.
+
+Lemma proof_of_cycpattern_check_entail_wit_8 : cycpattern_check_entail_wit_8.
+Proof.
+  right; pre_process; entailer!.
+  - unfold string_length in *.
+    assert (Hi : 0 <= i <= Zlength b_l).
+    { unfold rotation_prefix_154 in PreH13;
+      destruct PreH13 as [Hi0 Hrest]; lia. }
+    rewrite rotate_at_154_length by exact Hi.
+    rewrite <- PreH11.
+    apply CharArray.full_to_undef_full.
+  - eapply (rotation_scan_state_154_step a_l b_l i
+              (rotate_at_154 b_l i) retval a0).
+    + exact PreH12.
+    + unfold string_length in PreH11; rewrite <- PreH11; exact PreH13.
+    + exact PreH1.
+    + exact PreH2.
+Qed.
+
+Lemma proof_of_cycpattern_check_entail_wit_9 : cycpattern_check_entail_wit_9.
+Proof.
+  right; pre_process; entailer!.
+  all: unfold rotation_scan_state_154 in PreH10;
+       destruct PreH10 as [[Hlo Hhi] Hnone].
+  - exact Hlo.
+  - unfold string_length in PreH9; lia.
+Qed.
+
+Lemma proof_of_cycpattern_check_return_wit_1 : cycpattern_check_return_wit_1.
+Proof.
+  unfold cycpattern_check_return_wit_1; intros.
+  rewrite <- derivable1_orp_intros1.
+  assert (i = n) by lia; subst i.
+  assert (Hspec : problem_154_spec_z a_l b_l 0).
+  { apply rotation_scan_state_154_problem_spec; try assumption.
+    unfold string_length in PreH11; rewrite <- PreH11; exact PreH12. }
+  entailer!; unfold store_string; cancel.
+Qed.
+
+Lemma proof_of_cycpattern_check_return_wit_2 : cycpattern_check_return_wit_2.
+Proof.
+  unfold cycpattern_check_return_wit_2; intros.
+  rewrite <- derivable1_orp_intros2.
+  assert (Hspec : problem_154_spec_z a_l b_l 1).
+  { exact (rotation_success_154_problem_spec a_l b_l i
+             (rotate_at_154 b_l i) PreH6 PreH7 PreH10). }
+  entailer!; unfold store_string; cancel.
+Qed.
+
+Lemma proof_of_cycpattern_check_partial_solve_wit_5_pure :
+  cycpattern_check_partial_solve_wit_5_pure.
+Proof.
+  right; pre_process; entailer!.
+  unfold string_length in *.
+  assert (Hi : 0 <= i <= Zlength b_l).
+  { unfold rotation_prefix_154 in PreH15;
+    destruct PreH15 as [Hi0 Hrest]; lia. }
+  rewrite rotate_at_154_length by exact Hi.
+  lia.
+Qed.
