QCP_examples/humaneval/spec_logic_rewrite_c_files/coins_154.v
@@ -1,0 +1,554 @@
+Require Import Coq.ZArith.ZArith.
+Require Import Coq.Bool.Bool.
+Require Import Coq.Lists.List.
+Require Import Coq.Strings.Ascii.
+Require Import Coq.Strings.String.
+Require Import Coq.micromega.Lia.
+From AUXLib Require Import ListLib.
+From SimpleC.StdLib Require Import string_lib.
+
+Load "../spec/154".
+
+Import ListNotations.
+Local Open Scope Z_scope.
+
+Definition ascii_of_z_154 (z : Z) : ascii :=
+  ascii_of_N (Z.to_N z).
+
+Fixpoint string_of_list_z_154 (l : list Z) : string :=
+  match l with
+  | [] => EmptyString
+  | z :: tl => String (ascii_of_z_154 z) (string_of_list_z_154 tl)
+  end.
+
+Definition bool_of_z_154 (z : Z) : bool := Z.eqb z 1.
+
+Definition problem_154_pre_z (a b : list Z) : Prop :=
+  problem_154_pre (string_of_list_z_154 a) (string_of_list_z_154 b).
+
+Definition problem_154_spec_z (a b : list Z) (res : Z) : Prop :=
+  problem_154_spec
+    (string_of_list_z_154 a)
+    (string_of_list_z_154 b)
+    (bool_of_z_154 res).
+
+Definition rotate_at_154 (b : list Z) (i : Z) : list Z :=
+  sublist i (Zlength b) b ++ sublist 0 i b.
+
+Definition rotation_prefix_154
+    (b : list Z) (i j : Z) (out : list Z) : Prop :=
+  0 <= i < Zlength b /\
+  0 <= j <= Zlength b /\
+  out = sublist 0 j (rotate_at_154 b i).
+
+Definition rotation_scan_state_154
+    (a b : list Z) (i : Z) : Prop :=
+  0 <= i <= Zlength b /\
+  forall r out,
+    0 <= r < i ->
+    rotation_prefix_154 b r (Zlength b) out ->
+    forall pos, 0 <= pos <= Zlength a -> ~ substring_at a out pos.
+
+Definition rotation_success_154
+    (a b : list Z) (i : Z) (out : list Z) : Prop :=
+  rotation_prefix_154 b i (Zlength b) out /\
+  exists pos, substring_at a out pos.
+
+Lemma rotate_at_154_length : forall b i,
+  0 <= i <= Zlength b ->
+  Zlength (rotate_at_154 b i) = Zlength b.
+Proof.
+  intros b i Hi.
+  unfold rotate_at_154.
+  rewrite Zlength_app.
+  rewrite !Zlength_sublist by lia.
+  lia.
+Qed.
+
+Lemma rotation_prefix_154_zero : forall b i,
+  0 <= i < Zlength b ->
+  rotation_prefix_154 b i 0 [].
+Proof.
+  intros b i Hi.
+  unfold rotation_prefix_154.
+  repeat split; try lia.
+Qed.
+
+Lemma rotate_at_154_Znth : forall b i j,
+  0 <= i < Zlength b ->
+  0 <= j < Zlength b ->
+  Znth j (rotate_at_154 b i) 0 =
+  Znth ((i + j) mod Zlength b) b 0.
+Proof.
+  intros b i j Hi Hj.
+  unfold rotate_at_154.
+  assert (Hlen1 : Zlength (sublist i (Zlength b) b) = Zlength b - i).
+  { rewrite Zlength_sublist by lia. lia. }
+  destruct (Z_lt_ge_dec j (Zlength b - i)) as [Hleft | Hright].
+  - rewrite app_Znth1 by lia.
+    rewrite Znth_sublist by lia.
+    rewrite Z.mod_small by lia.
+    f_equal; lia.
+  - rewrite app_Znth2 by lia.
+    rewrite Hlen1.
+    rewrite Znth_sublist by lia.
+    assert (Hmod : (i + j) mod Zlength b = i + j - Zlength b).
+    { replace (i + j) with ((i + j - Zlength b) + 1 * Zlength b) by lia.
+      rewrite Z.mod_add by lia.
+      rewrite Z.mod_small by lia.
+      lia. }
+    rewrite Hmod.
+    f_equal; lia.
+Qed.
+
+Lemma rotation_prefix_154_step : forall b i j out ch,
+  rotation_prefix_154 b i j out ->
+  j < Zlength b ->
+  ch = Znth ((i + j) mod Zlength b) b 0 ->
+  rotation_prefix_154 b i (j + 1) (out ++ [ch]).
+Proof.
+  intros b i j out ch Hpref Hj Hch.
+  unfold rotation_prefix_154 in *.
+  destruct Hpref as [Hi [Hjb Hout]].
+  repeat split; try lia.
+  subst out.
+  rewrite (sublist_split 0 (j + 1) j (rotate_at_154 b i)) by
+      (try lia; rewrite rotate_at_154_length; lia).
+  rewrite (sublist_single 0 j (rotate_at_154 b i)) by
+      (rewrite rotate_at_154_length; lia).
+  rewrite rotate_at_154_Znth by lia.
+  now subst ch.
+Qed.
+
+Lemma all_ascii_rotate_at_154 : forall b i,
+  all_ascii b ->
+  0 <= i <= Zlength b ->
+  all_ascii (rotate_at_154 b i).
+Proof.
+  intros b i Hall Hi k Hk.
+  destruct (Z.eq_dec i (Zlength b)) as [-> | Hne].
+  - assert (Hkb : 0 <= k < Zlength b).
+    { rewrite rotate_at_154_length in Hk by lia; exact Hk. }
+    unfold rotate_at_154.
+    rewrite sublist_self by reflexivity.
+    assert (Hempty : sublist (Zlength b) (Zlength b) b = []).
+    { apply length_zero_iff_nil.
+      pose proof (Zlength_sublist (Zlength b) (Zlength b) b ltac:(lia)).
+      rewrite Zlength_correct in H; lia. }
+    rewrite Hempty; simpl.
+    apply Hall; exact Hkb.
+  - assert (Hkb : 0 <= k < Zlength b).
+    { rewrite rotate_at_154_length in Hk by lia; exact Hk. }
+    rewrite rotate_at_154_Znth by lia.
+    apply Hall.
+    apply Z.mod_pos_bound; lia.
+Qed.
+
+Lemma no_inner_nul_rotate_at_154 : forall b i,
+  no_inner_nul b ->
+  0 <= i <= Zlength b ->
+  no_inner_nul (rotate_at_154 b i).
+Proof.
+  intros b i Hnul Hi k Hk.
+  destruct (Z.eq_dec i (Zlength b)) as [-> | Hne].
+  - assert (Hkb : 0 <= k < Zlength b).
+    { rewrite rotate_at_154_length in Hk by lia; exact Hk. }
+    unfold rotate_at_154.
+    rewrite sublist_self by reflexivity.
+    assert (Hempty : sublist (Zlength b) (Zlength b) b = []).
+    { apply length_zero_iff_nil.
+      pose proof (Zlength_sublist (Zlength b) (Zlength b) b ltac:(lia)).
+      rewrite Zlength_correct in H; lia. }
+    rewrite Hempty; simpl.
+    apply Hnul; exact Hkb.
+  - assert (Hkb : 0 <= k < Zlength b).
+    { rewrite rotate_at_154_length in Hk by lia; exact Hk. }
+    rewrite rotate_at_154_Znth by lia.
+    apply Hnul.
+    apply Z.mod_pos_bound; lia.
+Qed.
+
+Lemma valid_string_rotate_at_154 : forall b i,
+  valid_string b ->
+  0 <= i <= Zlength b ->
+  valid_string (rotate_at_154 b i).
+Proof.
+  intros b i [Hall Hnul] Hi; split.
+  - now apply all_ascii_rotate_at_154.
+  - now apply no_inner_nul_rotate_at_154.
+Qed.
+
+Lemma rotation_scan_state_154_zero : forall a b,
+  rotation_scan_state_154 a b 0.
+Proof.
+  intros a b.
+  unfold rotation_scan_state_154.
+  split; [pose proof (Zlength_nonneg b); lia |].
+  intros r out Hr; lia.
+Qed.
+
+Lemma strstr_result_154_success : forall a out ret base,
+  ret <> 0 ->
+  strstr_result a out ret base ->
+  exists pos, substring_at a out pos.
+Proof.
+  intros a out ret base Hret Hstr.
+  unfold strstr_result in Hstr.
+  destruct Hstr as [[pos [Hsub [_ [_ Hnz]]]] | [_ Hzero]].
+  - now exists pos.
+  - contradiction.
+Qed.
+
+Lemma rotation_scan_state_154_step : forall a b i out ret base,
+  rotation_scan_state_154 a b i ->
+  rotation_prefix_154 b i (Zlength b) out ->
+  ret = 0 ->
+  strstr_result a out ret base ->
+  rotation_scan_state_154 a b (i + 1).
+Proof.
+  intros a b i out ret base Hscan Hpref Hret Hstr.
+  pose proof Hpref as Hpref_bounds.
+  unfold rotation_prefix_154 in Hpref_bounds.
+  destruct Hpref_bounds as [Hib _].
+  unfold rotation_scan_state_154 in *.
+  destruct Hscan as [Hi Hprev].
+  split; [lia |].
+  intros r rot Hr Hrot pos Hpos.
+  destruct (Z_lt_ge_dec r i) as [Hlt | Hge].
+  - eapply Hprev; eauto; lia.
+  - assert (r = i) by lia; subst r.
+    unfold strstr_result in Hstr.
+    destruct Hstr as [[p [_ [_ [_ Hnz]]]] | [Hnone Hzero]].
+    + lia.
+    + subst ret.
+      assert (rot = out).
+      { unfold rotation_prefix_154 in Hrot, Hpref.
+        destruct Hrot as [_ [_ ->]].
+        destruct Hpref as [_ [_ ->]].
+        reflexivity. }
+      subst rot.
+      eapply Hnone; eauto.
+Qed.
+
+Definition ascii_list_154 (l : list Z) : list ascii :=
+  map ascii_of_z_154 l.
+
+Lemma list_ascii_of_string_of_list_z_154 : forall l,
+  list_ascii_of_string (string_of_list_z_154 l) = ascii_list_154 l.
+Proof.
+  induction l as [|z tl IH]; simpl; auto.
+  now rewrite IH.
+Qed.
+
+Lemma Zlength_map_154 : forall {A B : Type} (f : A -> B) l,
+  Zlength (map f l) = Zlength l.
+Proof.
+  intros A B f l.
+  rewrite !Zlength_correct, map_length; reflexivity.
+Qed.
+
+Lemma map_sublist_154 : forall {A B : Type} (f : A -> B) lo hi l,
+  map f (sublist lo hi l) = sublist lo hi (map f l).
+Proof.
+  intros A B f lo hi l.
+  unfold sublist.
+  rewrite firstn_map, skipn_map.
+  reflexivity.
+Qed.
+
+Lemma Znth_ascii_list_154 : forall l i,
+  Znth i (ascii_list_154 l) (ascii_of_z_154 0) =
+  ascii_of_z_154 (Znth i l 0).
+Proof.
+  intros l i.
+  unfold ascii_list_154, Znth.
+  apply map_nth.
+Qed.
+
+Lemma ascii_of_z_154_inj_range : forall x y,
+  0 <= x <= 127 ->
+  0 <= y <= 127 ->
+  ascii_of_z_154 x = ascii_of_z_154 y ->
+  x = y.
+Proof.
+  intros x y Hx Hy Heq.
+  unfold ascii_of_z_154 in Heq.
+  apply (f_equal N_of_ascii) in Heq.
+  assert (HxN : (Z.to_N x < 256)%N).
+  { change (Z.to_N x < Z.to_N 256)%N.
+    apply (proj1 (Z2N.inj_lt x 256 ltac:(lia) ltac:(lia))); lia. }
+  assert (HyN : (Z.to_N y < 256)%N).
+  { change (Z.to_N y < Z.to_N 256)%N.
+    apply (proj1 (Z2N.inj_lt y 256 ltac:(lia) ltac:(lia))); lia. }
+  rewrite (N_ascii_embedding (Z.to_N x) HxN) in Heq.
+  rewrite (N_ascii_embedding (Z.to_N y) HyN) in Heq.
+  eapply Z2N.inj; eauto; lia.
+Qed.
+
+Lemma all_ascii_sublist_154 : forall l lo hi,
+  all_ascii l ->
+  0 <= lo <= hi ->
+  hi <= Zlength l ->
+  all_ascii (sublist lo hi l).
+Proof.
+  intros l lo hi Hall Hlo Hhi k Hk.
+  rewrite Zlength_sublist in Hk by lia.
+  rewrite Znth_sublist by lia.
+  apply Hall.
+  lia.
+Qed.
+
+Lemma ascii_list_154_inj : forall l1 l2,
+  all_ascii l1 ->
+  all_ascii l2 ->
+  ascii_list_154 l1 = ascii_list_154 l2 ->
+  l1 = l2.
+Proof.
+  intros l1 l2 H1 H2 Hmap.
+  apply (proj2 (list_eq_ext l1 l2 0)).
+  split.
+  - apply (f_equal (@Zlength ascii)) in Hmap.
+    unfold ascii_list_154 in Hmap.
+    rewrite !Zlength_map_154 in Hmap; exact Hmap.
+  - intros i Hi.
+    apply ascii_of_z_154_inj_range.
+    + apply H1; exact Hi.
+    + apply H2.
+      apply (f_equal (@Zlength ascii)) in Hmap.
+      unfold ascii_list_154 in Hmap.
+      rewrite !Zlength_map_154 in Hmap; lia.
+    + rewrite <- !Znth_ascii_list_154.
+      now rewrite Hmap.
+Qed.
+
+Lemma substring_at_154_to_is_substring : forall main sub pos,
+  substring_at main sub pos ->
+  is_substring (ascii_list_154 sub) (ascii_list_154 main).
+Proof.
+  intros main sub pos Hsub.
+  unfold substring_at in Hsub.
+  destruct Hsub as [Hpos [Hfit Hpoint]].
+  unfold string_length in Hpos, Hfit, Hpoint.
+  pose proof (Zlength_nonneg sub) as Hsub_len.
+  assert (Hmiddle : sublist pos (pos + Zlength sub) main = sub).
+  { apply (proj2 (list_eq_ext (sublist pos (pos + Zlength sub) main) sub 0)).
+    split.
+    - assert (Hbounds : 0 <= pos <= pos + Zlength sub /\
+                         pos + Zlength sub <= Zlength main) by (repeat split; lia).
+      rewrite (Zlength_sublist pos (pos + Zlength sub) main Hbounds); lia.
+    - intros k Hk.
+      assert (Hbounds : 0 <= pos <= pos + Zlength sub /\
+                         pos + Zlength sub <= Zlength main) by (repeat split; lia).
+      rewrite Zlength_sublist in Hk by exact Hbounds.
+      rewrite Znth_sublist by lia.
+      replace (k + pos) with (pos + k) by lia.
+      apply Hpoint; lia. }
+  assert (Hdecomp :
+      main = sublist 0 pos main ++ sub ++
+             sublist (pos + Zlength sub) (Zlength main) main).
+  { transitivity (sublist 0 (Zlength main) main).
+    - symmetry; apply sublist_self; reflexivity.
+    - rewrite (sublist_split 0 (Zlength main) pos main) by lia.
+      rewrite (sublist_split pos (Zlength main) (pos + Zlength sub) main) by lia.
+      rewrite Hmiddle, app_assoc; reflexivity. }
+  exists (ascii_list_154 (sublist 0 pos main)).
+  exists (ascii_list_154 (sublist (pos + Zlength sub) (Zlength main) main)).
+  unfold ascii_list_154.
+  rewrite Hdecomp at 1.
+  rewrite !map_app; reflexivity.
+Qed.
+
+Lemma rotate_at_154_is_rotation : forall b i,
+  0 <= i <= Zlength b ->
+  is_rotation_of (ascii_list_154 (rotate_at_154 b i)) (ascii_list_154 b).
+Proof.
+  intros b i Hi.
+  exists (ascii_list_154 (sublist 0 i b)).
+  exists (ascii_list_154 (sublist i (Zlength b) b)).
+  split.
+  - unfold ascii_list_154.
+    rewrite <- map_app.
+    f_equal.
+    rewrite <- (sublist_split 0 (Zlength b) i b) by lia.
+    symmetry; apply sublist_self; reflexivity.
+  - unfold ascii_list_154, rotate_at_154.
+    now rewrite map_app.
+Qed.
+
+Lemma rotation_success_154_problem_spec : forall a b i out,
+  valid_string a ->
+  valid_string b ->
+  rotation_success_154 a b i out ->
+  problem_154_spec_z a b 1.
+Proof.
+  intros a b i out Hva Hvb Hsuccess.
+  destruct Hsuccess as [Hpref [pos Hsub]].
+  unfold rotation_prefix_154 in Hpref.
+  destruct Hpref as [Hi [_ Hout]].
+  rewrite sublist_self in Hout by
+      (rewrite rotate_at_154_length; lia).
+  subst out.
+  unfold problem_154_spec_z, problem_154_spec, bool_of_z_154.
+  rewrite !list_ascii_of_string_of_list_z_154.
+  simpl.
+  split.
+  - intros _.
+    split.
+    + unfold ascii_list_154.
+      intro Hnil.
+      apply map_eq_nil in Hnil.
+      subst b; rewrite Zlength_nil in Hi; lia.
+    + exists (ascii_list_154 (rotate_at_154 b i)).
+      split.
+      * apply rotate_at_154_is_rotation; lia.
+      * now apply (substring_at_154_to_is_substring a (rotate_at_154 b i) pos).
+  - intros _; reflexivity.
+Qed.
+
+Lemma is_substring_154_to_substring_at : forall main sub,
+  all_ascii main ->
+  all_ascii sub ->
+  is_substring (ascii_list_154 sub) (ascii_list_154 main) ->
+  exists pos, substring_at main sub pos.
+Proof.
+  intros main sub Hmain Hsub [prefix [suffix Heq]].
+  set (pos := Zlength prefix).
+  assert (Hlen : Zlength (ascii_list_154 main) =
+                 Zlength prefix + Zlength (ascii_list_154 sub) + Zlength suffix).
+  { rewrite Heq, !Zlength_app; lia. }
+  unfold ascii_list_154 in Hlen.
+  rewrite !Zlength_map_154 in Hlen.
+  assert (Hpos : 0 <= pos) by (unfold pos; apply Zlength_nonneg).
+  assert (Hfit : pos + Zlength sub <= Zlength main).
+  { unfold pos; pose proof (Zlength_nonneg suffix); lia. }
+  assert (Hmiddle_ascii :
+      sublist pos (pos + Zlength sub) (ascii_list_154 main) =
+      ascii_list_154 sub).
+  { rewrite Heq.
+    rewrite (sublist_split_app_r pos (pos + Zlength sub) pos prefix
+              (ascii_list_154 sub ++ suffix)) by
+        (unfold pos; pose proof (Zlength_nonneg sub);
+         repeat split; try reflexivity; lia).
+    replace (pos - pos) with 0 by lia.
+    replace (pos + Zlength sub - pos) with (Zlength sub) by lia.
+    rewrite sublist_split_app_l by
+        (unfold ascii_list_154; rewrite ?Zlength_map_154;
+         pose proof (Zlength_nonneg sub); lia).
+    apply sublist_self.
+    unfold ascii_list_154; rewrite Zlength_map_154; reflexivity. }
+  assert (Hmiddle : sublist pos (pos + Zlength sub) main = sub).
+  { apply ascii_list_154_inj.
+    - apply all_ascii_sublist_154; [exact Hmain | | exact Hfit].
+      pose proof (Zlength_nonneg sub); lia.
+    - exact Hsub.
+    - unfold ascii_list_154 at 1.
+      rewrite map_sublist_154.
+      exact Hmiddle_ascii. }
+  exists pos.
+  unfold substring_at, string_length.
+  split.
+  - pose proof (Zlength_nonneg sub); lia.
+  - split; [exact Hfit |].
+  intros k Hk.
+  rewrite <- Hmiddle.
+  rewrite Znth_sublist by lia.
+  f_equal; lia.
+Qed.
+
+Lemma is_rotation_154_to_rotate_at : forall b rotated,
+  0 < Zlength b ->
+  is_rotation_of rotated (ascii_list_154 b) ->
+  exists i,
+    0 <= i < Zlength b /\
+    rotated = ascii_list_154 (rotate_at_154 b i).
+Proof.
+  intros b rotated Hb_nonempty [p1 [p2 [Hb Hrot]]].
+  unfold ascii_list_154 in Hb.
+  set (cut := Zlength p1).
+  assert (Hlength : Zlength b = Zlength p1 + Zlength p2).
+  { pose proof (f_equal (@Zlength ascii) Hb) as Hb_len.
+    rewrite Zlength_map_154, Zlength_app in Hb_len; lia. }
+  assert (Hcut : 0 <= cut <= Zlength b).
+  { unfold cut; pose proof (Zlength_nonneg p1); pose proof (Zlength_nonneg p2); lia. }
+  assert (Hp1 : p1 = ascii_list_154 (sublist 0 cut b)).
+  { unfold ascii_list_154.
+    rewrite map_sublist_154.
+    symmetry.
+    rewrite Hb.
+    rewrite sublist_split_app_l by (unfold cut; lia).
+    apply sublist_self; unfold cut; reflexivity. }
+  assert (Hp2 : p2 = ascii_list_154 (sublist cut (Zlength b) b)).
+  { unfold ascii_list_154.
+    rewrite map_sublist_154.
+    symmetry.
+    rewrite Hb.
+    rewrite (sublist_split_app_r cut (Zlength b) cut p1 p2) by
+        (unfold cut; repeat split; try reflexivity; lia).
+    replace (cut - cut) with 0 by lia.
+    replace (Zlength b - cut) with (Zlength p2) by (unfold cut; lia).
+    apply sublist_self; reflexivity. }
+  destruct (Z_lt_ge_dec cut (Zlength b)) as [Hproper | Hend].
+  - exists cut; split; [lia |].
+    rewrite Hrot, Hp1, Hp2.
+    unfold rotate_at_154, ascii_list_154.
+    now rewrite map_app.
+  - assert (Hp2_nil : p2 = []).
+    { destruct p2 as [|x xs]; [reflexivity |].
+      rewrite Zlength_cons in Hlength.
+      pose proof (Zlength_nonneg xs).
+      unfold cut in *; lia. }
+    exists 0; split; [lia |].
+    rewrite Hp2_nil in Hb, Hrot.
+    rewrite app_nil_r in Hb.
+    simpl in Hrot.
+    rewrite <- Hb in Hrot.
+    rewrite Hrot.
+    unfold rotate_at_154, ascii_list_154.
+    rewrite sublist_self by reflexivity.
+    unfold sublist; simpl; rewrite app_nil_r.
+    reflexivity.
+Qed.
+
+Lemma rotation_scan_state_154_problem_spec : forall a b,
+  valid_string a ->
+  valid_string b ->
+  rotation_scan_state_154 a b (Zlength b) ->
+  problem_154_spec_z a b 0.
+Proof.
+  intros a b Hva Hvb Hscan.
+  destruct Hva as [Haa Hna].
+  destruct Hvb as [Hab Hnb].
+  unfold problem_154_spec_z, problem_154_spec, bool_of_z_154.
+  rewrite !list_ascii_of_string_of_list_z_154.
+  simpl.
+  split.
+  - discriminate.
+  - intros [Hb_not_nil [rotated [Hrotation Hsubstring]]].
+    assert (Hb_pos : 0 < Zlength b).
+    { destruct b as [|x xs].
+      - exfalso; apply Hb_not_nil; reflexivity.
+      - rewrite Zlength_cons.
+        pose proof (Zlength_nonneg xs); lia. }
+    destruct (is_rotation_154_to_rotate_at b rotated Hb_pos Hrotation)
+      as [i [Hi Hrotated]].
+    subst rotated.
+    assert (Harot : all_ascii (rotate_at_154 b i)).
+    { apply all_ascii_rotate_at_154; [exact Hab | lia]. }
+    destruct (is_substring_154_to_substring_at
+                a (rotate_at_154 b i) Haa Harot Hsubstring)
+      as [pos Hsub].
+    unfold rotation_scan_state_154 in Hscan.
+    destruct Hscan as [_ Hnone].
+    assert (Hprefix : rotation_prefix_154 b i (Zlength b)
+                        (rotate_at_154 b i)).
+    { unfold rotation_prefix_154.
+      split; [exact Hi |].
+      split; [pose proof (Zlength_nonneg b); lia |].
+      rewrite sublist_self.
+      - reflexivity.
+      - symmetry; apply rotate_at_154_length; lia. }
+    exfalso.
+    eapply (Hnone i (rotate_at_154 b i) Hi Hprefix pos); eauto.
+    unfold substring_at, string_length in Hsub.
+    destruct Hsub as [Hpos _]; exact Hpos.
+Qed.
